WIP: global function table

theories/lang.v
@@ -1,1054 +1,46 @@
-From Equations Require Import Equations.
 From iris.program_logic Require Export language ectx_language ectxi_language.
-From stdpp Require Export strings binders gmap infinite.
 
-From stbor Require Export type.
+From stbor Require Export expr_semantics bor_semantics.
 
 Set Default Proof Using "Type".
 
-Module bor_lang.
-Open Scope Z_scope.
-
-(** Locations *)
-Definition block : Set := positive.
-Definition loc : Set := block * Z.
-
-Bind Scope loc_scope with loc.
-Delimit Scope loc_scope with L.
-Open Scope loc_scope.
-
-Definition shift_loc (l : loc) (z : Z) : loc := (l.1, l.2 + z).
-
-Notation "l +ₗ z" := (shift_loc l%L z%Z)
-  (at level 50, left associativity) : loc_scope.
-
-Notation ptr_id := nat (only parsing).
-Notation call_id := nat (only parsing).
-
-(** Stacked borrows *)
-Inductive tag :=
-  | Tagged (t: ptr_id)
-  | Untagged
-  .
-
-Instance tag_eq_dec : EqDecision tag.
-Proof. solve_decision. Defined.
-Instance tag_countable : Countable tag.
-Proof.
-  refine (inj_countable
-          (λ tg, match tg with
-              | Tagged t => inl t
-              | Untagged => inr ()
-              end)
-          (λ s, match s with
-              | inl t => Some $ Tagged t
-              | inr _ => Some $ Untagged
-              end) _); by intros [].
-Qed.
-
-Inductive permission := Unique | SharedReadWrite | SharedReadOnly | Disabled.
-Instance permission_eq_dec : EqDecision permission.
-Proof. solve_decision. Defined.
-Instance permission_countable : Countable permission.
-Proof.
-  refine (inj_countable
-    (λ p,
-      match p with
-      | Unique => 0 | SharedReadWrite => 1 | SharedReadOnly => 2 | Disabled => 3
-      end)
-    (λ s,
-      match s with
-      | 0 => Some Unique | 1 => Some SharedReadWrite | 2 => Some SharedReadOnly
-      | _ => Some Disabled
-      end) _); by intros [].
-Qed.
-
-(* Retag kinds *)
-Inductive retag_kind := FnEntry (c: call_id) | TwoPhase | RawRt | Default.
-Definition is_two_phase (kind: retag_kind) : bool :=
-  match kind with TwoPhase => true | _ => false end.
-Definition adding_protector (kind: retag_kind) : option call_id :=
-  match kind with FnEntry c => Some c | _ => None end.
-
-(* Protector tracker: track if a call_id is active, i.e. the call is still running *)
-Definition protectors := gmap call_id bool.
-
-(* Stacks of borrows. *)
-Record item := mkItem {
-  perm      : permission;
-  tg        : tag;
-  protector : option call_id;
-}.
-Instance item_eq_dec : EqDecision item.
-Proof. solve_decision. Defined.
-
-Definition stack := list item.
-Definition stacks := gmap loc stack.
-
-Implicit Type (α: stacks) (β: protectors) (t: ptr_id) (c: call_id) (T: type).
-
-(*** BASE SEMANTICS --------------------------------------------------------***)
-
-(** Unary/Binary ops *)
-Inductive bin_op :=
-  | AddOp     (* + addition       *)
-  | SubOp     (* - subtraction    *)
-(* | MulOp     (* * multiplication *)
-  | DivOp     (* / division       *)
-  | RemOp     (* % modulus        *)
-  | BitXorOp  (* ^ bit xor        *)
-  | BitAndOp  (* & bit and        *)
-  | BitOrOp   (* | bit or         *)
-  | ShlOp     (* << shift left    *)
-  | ShrOp     (* >> shift right   *) *)
-  | EqOp      (* == equality      *)
-  | LtOp      (* < less than      *)
-  | LeOp      (* <= less than or equal to *)
-(* | NeOp      (* != not equal to  *)
-  | GeOp      (* >= greater than or equal to *)
-  | GtOp      (* > greater than   *) *)
-  | OffsetOp  (* . offset         *)
-  .
-
-(** Base values *)
-Inductive lit := LitPoison | LitLoc (l: loc) (tg: tag) | LitInt (n : Z).
-
-Notation "[ ]" := (@nil binder) : binder_scope.
-Notation "a :: b" := (@cons binder a%binder b%binder)
-  (at level 60, right associativity) : binder_scope.
-Notation "[ x1 ; x2 ; .. ; xn ]" :=
-  (@cons binder x1%binder (@cons binder x2%binder
-        (..(@cons binder xn%binder (@nil binder))..))) : binder_scope.
-Notation "[ x ]" := (@cons binder x%binder (@nil binder)) : binder_scope.
-
-(** Expressions *)
-Inductive expr :=
-(* base values *)
-| Lit (l: lit)
-(* base lambda calculus *)
-| Var (x : string)
-| App (e : expr) (el: list expr)
-| Rec (f : binder) (xl : list binder) (e : expr)
-(* temp values *)
-| TVal (el: list expr)
-| Proj (e1 e2 : expr)
-| Conc (e1 e2: expr)
-(* bin op *)
-| BinOp (op : bin_op) (e1 e2 : expr)
-(* place operation *)
-| Place (l: loc) (tg: tag) (T: type)
-                                  (* A place is a tagged pointer: every access
-                                     to memory revolves around a place. *)
-| Deref (e: expr) (T: type)       (* Deference a pointer `e` into a place
-                                     presenting the location that `e` points to.
-                                     The location has type `T`. *)
-| Ref (e: expr)                   (* Turn a place `e` into a pointer value. *)
-| Field (e: expr) (path: list nat)(* Create a place that points to a component
-                                     of the place `e`. `path` defines the path
-                                     through the type. *)
-(* mem op *)
-| Copy (e : expr)                 (* Read from the place `e` *)
-| Write (e1 e2: expr)             (* Write the value `e2` to the place `e1` *)
-| Alloc (T: type)                 (* Allocate a place of type `T` *)
-| Free (e : expr)                 (* Free the place `e` *)
-(* atomic mem op *)
-| CAS (e0 e1 e2 : expr)           (* CAS the value `e2` for `e1` to the place `e0` *)
-| AtomWrite (e1 e2: expr)
-| AtomRead (e: expr)
-(* function call tracking *)
-| NewCall                         (* Issue a fresh id for the call *)
-| EndCall (e: expr)               (* End the call with id `e` *)
-(* retag *)
-| Retag (e : expr) (kind: retag_kind) (call_id: expr)
-                                  (* Retag the place `e` with retag kind `kind`. *)
-(* case *)
-| Case (e : expr) (el: list expr)
-(* concurrency *)
-(* | Fork (e : expr) *)
-(* observable behavior *)
-(* | SysCall (id: nat) *)
-.
-
-Bind Scope expr_scope with expr.
-Delimit Scope expr_scope with E.
-
-Arguments App _%E _%E.
-Arguments BinOp _ _%E _%E.
-Arguments TVal _%E.
-Arguments Proj _%E _%E.
-Arguments Conc _%E _%E.
-Arguments Deref _%E _%RustT.
-Arguments Ref _%E.
-Arguments Field _%E _.
-Arguments Copy _%E.
-Arguments Write _%E _%E.
-Arguments Alloc _%RustT.
-Arguments Free _%E.
-Arguments CAS _%E _%E _%E.
-Arguments AtomWrite _%E _%E.
-Arguments AtomRead _%E.
-Arguments Retag _%E _ _%E.
-Arguments Case _%E _%E.
-(* Arguments Fork _%E. *)
-
-(** Closedness *)
-Fixpoint is_closed (X : list string) (e : expr) : bool :=
-  match e with
-  | Lit _ | Place _ _ _ | Alloc _ | NewCall (* | SysCall _ *) => true
-  | Var x => bool_decide (x ∈ X)
-  | Rec f xl e => is_closed (f :b: xl +b+ X) e
-  | BinOp _ e1 e2 | AtomWrite e1 e2 | Write e1 e2 | Retag e1 _ e2
-    | Conc e1 e2 | Proj e1 e2 => is_closed X e1 && is_closed X e2
-  | TVal el => forallb (is_closed X) el
-  | App e el | Case e el => is_closed X e && forallb (is_closed X) el
-  | AtomRead e | Copy e | Deref e _ | Ref e | Field e _
-    | Free e | EndCall e (* | Fork e *) => is_closed X e
-  | CAS e0 e1 e2 => is_closed X e0 && is_closed X e1 && is_closed X e2
-  end.
-
-Class Closed (X : list string) (e : expr) := closed : is_closed X e.
-Instance closed_proof_irrel env e : ProofIrrel (Closed env e).
-Proof. rewrite /Closed. apply _. Qed.
-Instance closed_decision env e : Decision (Closed env e).
-Proof. rewrite /Closed. apply _. Qed.
-
-(** Heap values *)
-Inductive immediate :=
-| LitV (l : lit)
-| RecV (f : binder) (xl : list binder) (e : expr) `{Closed (f :b: xl +b+ []) e}.
-
-(** Irreducible (language values) *)
-Inductive val :=
-| ImmV (v : immediate)
-| TValV (vl : list immediate)
-| PlaceV (l: loc) (tg: tag) (T: type)
-.
-Bind Scope val_scope with val.
-Delimit Scope val_scope with V.
-
-Definition of_immediate (v: immediate) : expr :=
-  match v with
-  | LitV l => Lit l
-  | RecV f xl e => Rec f xl e
-  end.
-Definition to_immediate (e: expr): option immediate :=
-  match e with
-  | Rec f xl e =>
-    if decide (Closed (f :b: xl +b+ []) e) then Some (RecV f xl e) else None
-  | Lit l => Some (LitV l)
-  | _ => None
-  end.
-Definition to_immediates (vl : list immediate) (el: list expr)
-  : option (list immediate) :=
-  foldl (λ acc e, vl ← acc; v ← to_immediate e; Some (vl ++ [v])) (Some vl) el.
-
-Definition of_val (v : val) : expr :=
-  match v with
-  | ImmV v => of_immediate v
-  | TValV vl => TVal (of_immediate <$> vl)
-  | PlaceV l tag T => Place l tag T
-  end.
-Definition to_val (e : expr) : option val :=
-  match e with
-  | Rec _ _ _ | Lit _ => ImmV <$> (to_immediate e)
-  | Place l T tag => Some (PlaceV l T tag)
-  | TVal el => vl ← to_immediates [] el; Some (TValV vl)
-  | _ => None
-  end.
-
-(** Substitution *)
-Fixpoint subst (x : string) (es : expr) (e : expr) : expr :=
-  match e with
-  | Var y => if bool_decide (y = x) then es else Var y
-  | Lit l => Lit l
-  | Rec f xl e =>
-    Rec f xl $ if bool_decide (BNamed x ≠ f ∧ BNamed x ∉ xl) then subst x es e else e
-  | Place l tag T => Place l tag T
-  | App e1 el => App (subst x es e1) (map (subst x es) el)
-  | BinOp op e1 e2 => BinOp op (subst x es e1) (subst x es e2)
-  | TVal el => TVal (map (subst x es) el)
-  | Proj e1 e2 => Proj (subst x es e1) (subst x es e2)
-  | Conc e1 e2 => Conc (subst x es e1) (subst x es e2)
-  | Copy e => Copy (subst x es e)
-  | Write e1 e2 => Write (subst x es e1) (subst x es e2)
-  | Alloc T => Alloc T
-  | Free e => Free (subst x es e)
-  | CAS e0 e1 e2 => CAS (subst x es e0) (subst x es e1) (subst x es e2)
-  | AtomWrite e1 e2 => AtomWrite (subst x es e1) (subst x es e2)
-  | AtomRead e => AtomRead (subst x es e)
-  | Deref e T => Deref (subst x es e) T
-  | Ref e => Ref (subst x es e)
-  | Field e path => Field (subst x es e) path
-  | NewCall => NewCall
-  | EndCall e => EndCall (subst x es e)
-  | Retag e kind call => Retag (subst x es e) kind (subst x es call)
-  | Case e el => Case (subst x es e) (map (subst x es) el)
-  (* | Fork e => Fork (subst x es e) *)
-  (* | SysCall id => SysCall id *)
-  end.
-
-(* formal argument list substitution *)
-Definition subst' (mx : binder) (es : expr) : expr → expr :=
-  match mx with BNamed x => subst x es | BAnon => id end.
-
-Fixpoint subst_l (xl : list binder) (esl : list expr) (e : expr) : option expr :=
-  match xl, esl with
-  | [], [] => Some e
-  | x::xl, es::esl => subst' x es <$> subst_l xl esl e
-  | _, _ => None
-  end.
-Arguments subst_l _%binder _ _%E.
-
-Definition subst_v (xl : list binder) (vsl : vec val (length xl))
-                   (e : expr) : expr :=
-  Vector.fold_right2 (λ b, subst' b ∘ of_val) e _ (list_to_vec xl) vsl.
-Arguments subst_v _%binder _ _%E.
-
-Lemma subst_v_eq (xl : list binder) (vsl : vec val (length xl)) e :
-  Some $ subst_v xl vsl e = subst_l xl (of_val <$> vec_to_list vsl) e.
-Proof.
-  revert vsl. induction xl=>/= vsl; inv_vec vsl=>//=v vsl. by rewrite -IHxl.
-Qed.
-
-(** Evaluation contexts *)
-Inductive ectx_item :=
-| AppLCtx (el : list expr)
-| AppRCtx (v : val) (vl : list val) (el : list expr)
-| BinOpLCtx (op : bin_op) (e2 : expr)
-| BinOpRCtx (op : bin_op) (v1 : val)
-| TValCtx (vl : list val) (el : list expr)
-| ProjLCtx (e : expr)
-| ProjRCtx (v : val)
-| ConcLCtx (e : expr)
-| ConcRCtx (v : val)
-| CopyCtx
-| WriteLCtx (e : expr)
-| WriteRCtx (v : val)
-| FreeCtx
-| CasLCtx (e1 e2: expr)
-| CasMCtx (v0 : val) (e2 : expr)
-| CasRCtx (v0 : val) (v1 : val)
-| AtRdCtx
-| AtWrLCtx (e : expr)
-| AtWrRCtx (v : val)
-| DerefCtx (T: type)
-| RefCtx
-| FieldCtx (path : list nat)
-| EndCallCtx
-| RetagLCtx (kind: retag_kind) (call: expr)
-| RetagRCtx (v: val) (kind: retag_kind)
-| CaseCtx (el : list expr).
-
-Definition fill_item (Ki : ectx_item) (e : expr) : expr :=
-  match Ki with
-  | AppLCtx el => App e el
-  | AppRCtx v vl el => App (of_val v) ((of_val <$> vl) ++ e :: el)
-  | BinOpLCtx op e2 => BinOp op e e2
-  | BinOpRCtx op v1 => BinOp op (of_val v1) e
-  | TValCtx vl el => TVal ((of_val <$> vl) ++ e :: el)
-  | ProjLCtx e2 => Proj e e2
-  | ProjRCtx v1 => Proj (of_val v1) e
-  | ConcLCtx e2 => Conc e e2
-  | ConcRCtx v1 => Conc (of_val v1) e
-  | CopyCtx => Copy e
-  | WriteLCtx e2 => Write e e2
-  | WriteRCtx v1 => Write (of_val v1) e
-  | FreeCtx => Free e
-  | CasLCtx e1 e2 => CAS e e1 e2
-  | CasMCtx v0 e2 => CAS (of_val v0) e e2
-  | CasRCtx v0 v1 => CAS (of_val v0) (of_val v1) e
-  | AtRdCtx => AtomRead e
-  | AtWrLCtx e2 => AtomWrite e e2
-  | AtWrRCtx v1 => AtomWrite (of_val v1) e
-  | DerefCtx T => Deref e T
-  | RefCtx => Ref e
-  | FieldCtx path => Field e path
-  | EndCallCtx => EndCall e
-  | RetagLCtx kind call => Retag e kind call
-  | RetagRCtx v kind => Retag (of_val v) kind e
-  | CaseCtx el => Case e el
-  end.
-
-(** Main state: a heap of immediates. *)
-Definition mem := gmap loc immediate.
-Implicit Type (h: mem).
-
-(** The stepping relation *)
-(* Be careful to make sure that poison is always stuck when used for anything
-   except for reading from or writing to memory! *)
-Definition Z_of_bool (b : bool) : Z :=
-  if b then 1 else 0.
-
-Definition lit_of_bool (b : bool) : lit :=
-  LitInt $ Z_of_bool b.
-
-Fixpoint init_mem (l:loc) (n:nat) h : mem :=
-  match n with
-  | O => h
-  | S n => <[l:=LitV LitPoison]>(init_mem (l +ₗ 1) n h)
-  end.
-
-Fixpoint free_mem (l:loc) (n:nat) h : mem :=
-  match n with
-  | O => h
-  | S n => delete l (free_mem (l +ₗ 1) n h)
-  end.
-
-Inductive lit_eq h : lit → lit → Prop :=
-(* No refl case for poison *)
-| IntRefl z : lit_eq h (LitInt z) (LitInt z)
-| LocRefl l tag1 tag2 : lit_eq h (LitLoc l tag1) (LitLoc l tag2)
-(* Comparing unallocated pointers can non-deterministically say they are equal
-   even if they are not.  Given that our `free` actually makes addresses
-   re-usable, this may not be strictly necessary, but it is the most
-   conservative choice that avoids UB (and we cannot use UB as this operation is
-   possible in safe Rust).  See
-   <https://internals.rust-lang.org/t/comparing-dangling-pointers/3019> for some
-   more background. *)
-| LocUnallocL l1 l2 tag1 tag2 :
-    h !! l1 = None →
-    lit_eq h (LitLoc l1 tag1) (LitLoc l2 tag2)
-| LocUnallocR l1 l2 tag1 tag2 :
-    h !! l2 = None →
-    lit_eq h (LitLoc l1 tag1) (LitLoc l2 tag2).
-
-Inductive lit_neq : lit → lit → Prop :=
-| IntNeq z1 z2 :
-    z1 ≠ z2 → lit_neq (LitInt z1) (LitInt z2)
-| LocNeq l1 l2 tag1 tag2 :
-    l1 ≠ l2 → lit_neq (LitLoc l1 tag1) (LitLoc l2 tag2)
-| LocNeqNullR l tag :
-    lit_neq (LitLoc l tag) (LitInt 0)
-| LocNeqNullL l tag :
-    lit_neq (LitInt 0) (LitLoc l tag).
-
-Inductive bin_op_eval h : bin_op → lit → lit → lit → Prop :=
-| BinOpPlus z1 z2 :
-    bin_op_eval h AddOp (LitInt z1) (LitInt z2) (LitInt (z1 + z2))
-| BinOpMinus z1 z2 :
-    bin_op_eval h SubOp (LitInt z1) (LitInt z2) (LitInt (z1 - z2))
-| BinOpLe z1 z2 :
-    bin_op_eval h LeOp (LitInt z1) (LitInt z2) (lit_of_bool $ bool_decide (z1 ≤ z2))
-| BinOpLt z1 z2 :
-    bin_op_eval h LtOp (LitInt z1) (LitInt z2) (lit_of_bool $ bool_decide (z1 < z2))
-| BinOpEqTrue l1 l2 :
-    lit_eq h l1 l2 → bin_op_eval h EqOp l1 l2 (lit_of_bool true)
-| BinOpEqFalse l1 l2 :
-    lit_neq l1 l2 → bin_op_eval h EqOp l1 l2 (lit_of_bool false)
-| BinOpOffset l z tag :
-    bin_op_eval h OffsetOp (LitLoc l tag) (LitInt z) (LitLoc (l +ₗ z) tag).
-
-Definition stuck_term := App (Lit $ LitInt 0) [].
-
-Inductive event :=
-| AllocEvt (l : loc) (lbor: tag) (T: type)
-| DeallocEvt (l: loc) (lbor: tag) (T: type)
-| CopyEvt (l: loc) (lbor: tag) (T: type) (vl: list immediate)
-| WriteEvt (l: loc) (lbor: tag) (T: type) (vl: list immediate)
-| NewCallEvt (call: call_id)
-| EndCallEvt (call: call_id)
-| RetagEvt (x: loc) (T: type) (kind: retag_kind)
-(* | SysCallEvt (id: nat) *)
-| SilentEvt
-.
-
-(* Compute subtype of `T` and offset to it from `path` *)
-Fixpoint field_access (T: type) (path : list nat) :
-  option (nat * type) :=
-  match path with
-  | [] => Some (O, T)
-  | i :: path =>
-    match T with
-    | Scalar sz => if decide (i ≤ sz) then Some (i, Scalar (sz - i)) else None
-    | Reference _ _ => match i with O => Some (O, T) | _ => None end
-    | Unsafe T => field_access T path
-    | Union Ts => T ← Ts !! i ; field_access T path
-    | Product Ts =>
-        T ← Ts !! i ; offT ← field_access T path;
-        let sz : nat := foldl (λ sz T', sz + tsize T')%nat O (take i Ts) in
-        Some (offT.1 + sz, offT.2)%nat
-    | Sum Ts =>
-        T ← Ts !! i ; offT ← field_access T path; Some (offT.1 + 1, offT.2)%nat
-    end
-  end.
-
-Fixpoint write_mem l (vl: list immediate) h: mem :=
-  match vl with
-  | [] => h
-  | v :: vl => write_mem (l +ₗ 1) vl (<[l := v]> h)
-  end.
-
-Equations read_mem (l: loc) (n: nat) (h: mem) : option (list immediate) :=
-  read_mem l n h := go l n (Some [])
-  where go : loc → nat → option (list immediate) → option (list immediate) :=
-        go l O      oacc := oacc;
-        go l (S n)  oacc :=
-          acc ← oacc ;
-          v ← h !! l;
-          go (l +ₗ 1) n (Some (acc ++ [v])).
-
-Inductive base_step :
-  expr → mem → event → expr → mem → list expr → Prop :=
-| BinOpBS op l1 l2 l' h :
-    bin_op_eval h op l1 l2 l' →
-    base_step (BinOp op (TVal [Lit l1]) (TVal [Lit l2])) h
-              SilentEvt (TVal [Lit l']) h []
-| BetaBS f xl e e' el h :
-    Forall (λ ei, is_Some (to_val ei)) el →
-    Closed (f :b: xl +b+ []) e →
-    subst_l (f::xl) (Rec f xl e :: el) e = Some e' →
-    base_step (App (Rec f xl e) el) h SilentEvt e' h []
-(* TODO: add more operations for tempvalue lists *)
-| ProjBS h el i vl v
-    (DEFINED: 0 ≤ i ∧ vl !! (Z.to_nat i) = Some v)
-    (VALUES: to_val (TVal el) = Some (TValV vl)) :
-    base_step (Proj (TVal el) (Lit $ LitInt i)) h SilentEvt (of_val (ImmV v)) h []
-| ConcBS h el1 el2 vl1 vl2
-    (VALUES1: to_val (TVal el1) = Some (TValV vl1))
-    (VALUES2: to_val (TVal el2) = Some (TValV vl2)):
-    base_step (Conc (TVal el1) (TVal el2)) h
-              SilentEvt (of_val (TValV (vl1 ++ vl2))) h []
-| CopyBS l lbor T (vl: list immediate) h
-    (READ: read_mem l (tsize T) h = Some vl)
-    (* (LEN: length vl = tsize T)
-    (VALUES: ∀ (i: nat), (i < length vl)%nat → h !! (l +ₗ i) = vl !! i) *) :
-    base_step (Copy (Place l lbor T)) h
-              (CopyEvt l lbor T vl)
-              (of_val (TValV vl)) h
-              []
-| WriteBS l lbor T el vl h (LENe: length vl = tsize T)
-    (DEFINED: ∀ (i: nat), (i < length vl)%nat → l +ₗ i ∈ dom (gset loc) h)
-    (VALUES: to_val (TVal el) = Some (TValV vl)) :
-    base_step (Write (Place l lbor T) (TVal el)) h
-              (WriteEvt l lbor T vl)
-              (Lit LitPoison) (write_mem l vl h)
-              []
-| AllocBS l lbor T h :
-    (∀ m, h !! (l +ₗ m) = None) →
-    base_step (Alloc T) h
-              (AllocEvt l lbor T)
-              (Place l lbor T) (init_mem l (tsize T) h)
-              []
-| DeallocBS T l lbor h :
-    (∀ m, is_Some (h !! (l +ₗ m)) ↔ 0 ≤ m < tsize T) →
-    base_step (Free (Place l lbor T)) h
-              (DeallocEvt l lbor T)
-              (Lit LitPoison) (free_mem l (tsize T) h)
-              []
-| NewCallBS call h:
-    base_step NewCall h (NewCallEvt call) (Lit $ LitInt call) h []
-| EndCallBS (call: Z) h:
-    (0 ≤ Z.to_nat call)%nat →
-    base_step (EndCall (Lit $ LitInt call)) h
-              (EndCallEvt (Z.to_nat call)) (Lit LitPoison) h []
-| RefBS l lbor T h :
-    is_Some (h !! l) →
-    base_step (Ref (Place l lbor T)) h SilentEvt (Lit (LitLoc l lbor)) h []
-| DerefBS l lbor T h
-    (DEFINED: ∀ (i: nat), (i < tsize T)%nat → l +ₗ i ∈ dom (gset loc) h) :
-    base_step (Deref (Lit (LitLoc l lbor)) T) h
-              SilentEvt
-              (Place l lbor T) h
-              []
-| FieldBS l lbor T path off T' h
-    (FIELD: field_access T path = Some (off, T')) :
-    base_step (Field (Place l lbor T) path) h
-              SilentEvt (Place (l +ₗ off) lbor T') h []
-| RetagBS x xbor T kind kind' h e v
-    (VAL: to_val e = Some v)
-    (KIND: match kind with
-           | FnEntry _ => ∃ call, v = ImmV $ LitV $ LitInt call ∧
-                          0 ≤ call ∧ kind' = FnEntry (Z.to_nat call)
-           | _ => kind' = kind
-           end) :
-    base_step (Retag (Place x xbor T) kind e) h
-              (RetagEvt x T kind' ) (Lit LitPoison) h []
-| CaseBS i el e h :
-    0 ≤ i →
-    el !! (Z.to_nat i) = Some e →
-    base_step (Case (Lit $ LitInt i) el) h SilentEvt e h []
-(* | ForkBS e h:
-    base_step (Fork e) h SilentEvt (Lit LitPoison) h [e] *)
-(* observable behavior *)
-(* | SysCallBS id h:
-    base_step (SysCall id) h (SysCallEvt id) (Lit LitPoison) h [] *).
-
-(*** STACKED BORROWS SEMANTICS ---------------------------------------------***)
-
-(** CORE SEMANTICS *)
-
-Inductive access_kind := AccessRead | AccessWrite.
-
-Definition grants (perm: permission) (access: access_kind) : bool :=
-  match perm, access with
-  | Disabled, _ => false
-  (* All items grant read access.
-    All items except SharedReadOnly grant write access. *)
-  | SharedReadOnly, AccessWrite => false
-  | _, _ => true
-  end.
-
-Definition matched_grant (access: access_kind) (bor: tag) (it: item) :=
-  grants it.(perm) access ∧ it.(tg) = bor.
-Instance matched_grant_dec (access: access_kind) (bor: tag) :
-  Decision (matched_grant access bor it) := _.
-
-(* This is different from the implementation: left-to-right is top-to-bottom
-  of the stack. So 0 is top of the stack. The index returned by this function
-  also follows this scheme (smaller means higher in the stack). *)
-Definition find_granting (stk: stack) (access: access_kind) (bor: tag) :
-  option (nat * permission) :=
-  (λ nit, (nit.1, nit.2.(perm))) <$> (list_find (matched_grant access bor) stk).
-
-
-Definition is_active β (c: call_id) : bool :=
-  bool_decide (β !! c = Some true).
-Definition is_active_protector β (it: item) :=
-  match it.(protector) with
-  | Some c => β !! c = Some true
-  | _ => False
-  end.
-Instance is_active_protector_dec β : Decision (is_active_protector β it).
-Proof. intros it. rewrite /is_active_protector. case_match; solve_decision. Qed.
-
-(* Find the top active protector *)
-Definition find_top_active_protector β (stk: stack) :=
-  list_find (is_active_protector β) stk.
-(* Checks to deallocate a location: Like a write access, but also there must be
-  no active protectors at all. *)
-Definition dealloc1 (stk: stack) (bor: tag) β : option unit :=
-  (* Step 1: Find granting item. *)
-  found ← find_granting stk AccessWrite bor;
-  (* Step 2: Check that there are no active protectors left. *)
-  if find_top_active_protector β stk then None else Some ().
-
-(* Find the index RIGHT BEFORE the first incompatiable item *)
-Definition find_first_write_incompatible
-  (stk: stack) (pm: permission) : option nat :=
-  match pm with
-  | Unique => Some (length stk)
-  | SharedReadWrite =>
-      match (list_find (λ it, it.(perm) ≠ SharedReadWrite) (reverse stk)) with
-      | Some (idx, _) => Some ((length stk) - idx)%nat
-      | _ => Some O
-      end
-  | SharedReadOnly | Disabled => None
-  end.
-
-Definition check_protector β (it: item) : bool :=
-  match it.(protector) with
-  | None => true
-  | Some c => if is_active β c then false else true
-  end.
-
-(* Remove from `stk` the items before `idx`.
-  Check that removed items do not have active protectors.
-  The check is run from the top to before the `idx`. *)
-Fixpoint remove_check β (stk: stack) (idx: nat) : option stack :=
-  match idx, stk with
-  (* Assumption: idx ≤ length stk *)
-  | S _, [] => None
-  | O, stk => Some stk
-  | S idx, it :: stk =>
-      if check_protector β it then remove_check β stk idx else None
-  end.
-
-(* Replace any Unique permission with Disabled, starting from the top of the
-  stack. Check that replaced item do not have active protectors *)
-Fixpoint replace_check' β (acc stk : stack) : option stack :=
-  match stk with
-  | [] => Some acc
-  | it :: stk =>
-      if decide (it.(perm) = Unique) then
-        if check_protector β it
-        then let new := mkItem Disabled it.(tg) it.(protector) in
-             replace_check' β (acc ++ [new]) stk
-        else None
-      else replace_check' β (acc ++ [it]) stk
-  end.
-Definition replace_check β (stk: stack) : option stack :=
-  replace_check' β [] stk.
-
-(* Test if a memory `access` using pointer tagged `tg` is granted.
-   If yes, return the index (in the old stack) of the item that granted it,
-   as well as the new stack. *)
-Definition access1 (stk: stack) (access: access_kind) (tg: tag) β
-  : option (nat * stack) :=
-  (* Step 1: Find granting item. *)
-  idx_p ← find_granting stk access tg;
-  (* Step 2: Remove incompatiable items. *)
-  match access with
-  | AccessWrite =>
-      (* Remove everything above the write-compatible items, like a proper stack. *)
-      incompat_idx ← find_first_write_incompatible (take idx_p.1 stk) idx_p.2;
-      stk' ← remove_check β (take idx_p.1 stk) incompat_idx;
-      Some (idx_p.1, stk' ++ drop idx_p.1 stk)
-  | AccessRead =>
-      (* On a read, *disable* all `Unique` above the granting item. *)
-      stk' ← replace_check β (take idx_p.1 stk);
-      Some (idx_p.1, stk' ++ drop idx_p.1 stk)
-  end.
-
-(* Initialize [l, l + n) with singleton stacks of `tg` *)
-Fixpoint init_stacks α (l:loc) (n:nat) (tg: tag) : stacks :=
-  match n with
-  | O => α
-  | S n => <[l:= [mkItem Unique tg None]]>(init_stacks α (l +ₗ 1) n tg)
-  end.
-
-Fixpoint for_each α (l:loc) (n:nat) (dealloc: bool) (f: stack → option stack)
-  : option stacks :=
-  match n with
-  | O => Some α
-  | S n =>
-      let l' := (l +ₗ n) in
-      stk ← α !! l'; stk' ← f stk ;
-      if dealloc
-      then for_each (delete l' α) l n dealloc f
-      else for_each (<[l':=stk']> α) l n dealloc f
-  end.
-
-(* Perform the access check on a block of continuous memory.
- * This implements Stacks::memory_read/memory_written/memory_deallocated. *)
-Definition memory_read α β l (tg: tag) (n: nat) : option stacks :=
-  for_each α l n false (λ stk, nstk' ← access1 stk AccessRead tg β; Some nstk'.2).
-Definition memory_written α β l (tg: tag) (n: nat) : option stacks :=
-  for_each α l n false (λ stk, nstk' ← access1 stk AccessWrite tg β; Some nstk'.2).
-Definition memory_deallocated α β l (tg: tag) (n: nat) : option stacks :=
-  for_each α l n true (λ stk, dealloc1 stk tg β ;; Some []).
-
-Definition unsafe_action
-  {A: Type} (f: A → loc → nat → bool → option A) (a: A) (l: loc)
-  (last frozen_size unsafe_size: nat) :
-  option (A * (nat * nat)) :=
-  (* Anything between the last UnsafeCell and this UnsafeCell is frozen *)
-  a' ← f a (l +ₗ last) frozen_size true;
-  (* This UnsafeCell is not frozen *)
-  let cur_off := (last + frozen_size)%nat in
-    a'' ← f a' (l +ₗ cur_off) unsafe_size false ;
-    Some (a'', ((cur_off + unsafe_size)%nat, O))
-  .
-
-(** Reborrow *)
-
-(* visit the type left-to-right and apply the action `f`.
- + `last` is the offset of `l` from the last UnsafeCell,
- + `cur_dist` is the distance between `last` and the current offset of the
-   visit, which is also the start of the sub-type `T`.
- + a` of type A is the accumulator for the visit.
- When an UnsafeCell is found, the action `f` is applied twice, through
- `unsafe_action`:
- - First `f` is applied for the frozen block, which is the range
-   [last, last + cur_dist). `f` is applied with the boolean flag `true`
-   (for frozen).
- - Then `f` is applied for the unfrozen block, which is the range
-   [last + cur_dist, last + cur_dist + unsafe_block_size). `f` is applied with
-   the boolean flag `false`. *)
-Section blah.
-Context {A: Type}.
-Equations visit_freeze_sensitive'
-  (h: mem) (l: loc) (f: A → loc → nat → bool → option A)
-  (a: A) (last cur_dist: nat) (T: type) : option (A * (nat * nat)) :=
-  visit_freeze_sensitive' h l f a last cur_dist (Scalar n) :=
-    (* consider frozen, simply extend the distant by n *)
-      Some (a, (last, cur_dist + n)%nat) ;
-  visit_freeze_sensitive' h l f a last cur_dist (Reference _ _) :=
-    (* consider frozen, extend the distant by 1 *)
-      Some (a, (last, S cur_dist)) ;
-  visit_freeze_sensitive' h l f a last cur_dist (Unsafe T) :=
-    (* reach an UnsafeCell, apply the action `f` and return new `last` and
-        `cur_dist` *)
-      unsafe_action f a l last cur_dist (tsize T) ;
-  visit_freeze_sensitive' h l f a last cur_dist (Union Ts) :=
-    (* If it's a union, look at the type to see if there is UnsafeCell *)
-      if is_freeze (Union Ts)
-      (* No UnsafeCell, consider the whole block frozen and simply extend the
-          distant. *)
-      then Some (a, (last, cur_dist + (tsize (Union Ts)))%nat)
-      (* There can be UnsafeCell, consider the whole block unfrozen and perform
-          `f a _ _ false` on the whole block. `unsafe_action` will return the
-          offsets for the following visit. *)
-      else unsafe_action f a l last cur_dist (tsize (Union Ts)) ;
-  visit_freeze_sensitive' h l f a last cur_dist (Product Ts) :=
-    (* Try a shortcut *)
-      if is_freeze (Product Ts)
-      (* No UnsafeCell, consider the whole block frozen and simply extend the
-        distant. *)
-      then Some (a, (last, cur_dist + (tsize (Product Ts)))%nat)
-      (* This implements left-to-right search on the type, which guarantees
-        that the offsets are increasing. *)
-      else visit_LR a last cur_dist Ts
-        where visit_LR (a: A) (last cur_dist: nat) (Ts: list type)
-          : option (A * (nat * nat)) :=
-          { visit_LR a last cur_dist [] := Some (a, (last, cur_dist)) ;
-            visit_LR a last cur_dist (T :: Ts) :=
-              alc ← visit_freeze_sensitive' h l f a last cur_dist T ;
-              visit_LR alc.1 alc.2.1 alc.2.2 Ts } ;
-  visit_freeze_sensitive' h l f a last cur_dist (Sum Ts) :=
-    (* Try a shortcut *)
-      if is_freeze (Sum Ts)
-      (* No UnsafeCell, consider the whole block frozen and simply extend the
-          distant. *)
-      then Some (a, (last, cur_dist + (tsize (Sum Ts)))%nat)
-      else
-        match h !! (l +ₗ (last + cur_dist)) with
-        (* This looks up the current state to see which discriminant currently
-            is active (which is an integer) and redirect the visit for the type
-            of that discriminant. Note that this consitutes a read-access, and
-            should adhere to the access checks. But we are skipping them here.
-            FIXME *)
-        | Some (LitV (LitInt i)) =>
-            if decide (O ≤ i)
-            then (* the discriminant is well-defined, visit with the
-                    corresponding type *)
-              alc ← visit_lookup Ts (Z.to_nat i) ;
-              (* Anything in the padding is considered frozen and will be
-                 applied with the action by the following visit.
-                 `should_offset` presents the offset that the visit SHOULD
-                 arrive at after the visit. If there are padding bytes left,
-                 they will be added to the cur_dist. *)
-              let should_offset := (last + cur_dist + tsize (Sum Ts))%nat in
-                Some (alc.1, (alc.2.1, (should_offset - alc.2.1)%nat))
-            else None
-        | _ => None
-        end
-      where visit_lookup (Ts: list type) (i: nat) : option (A * (nat * nat)) :=
-            { visit_lookup [] _             := None ;
-              visit_lookup (T :: _) O      :=
-                visit_freeze_sensitive' h l f a last (S cur_dist) T ;
-              visit_lookup (T :: Ts) (S i)  := visit_lookup Ts i }
-  .
-End blah.
-
-Definition visit_freeze_sensitive {A: Type}
-  h (l: loc) (T: type) (f: A → loc → nat → bool → option A) (a: A) : option A :=
-  match visit_freeze_sensitive' h l f a O O T with
-  | Some (a', (last', cur_dist')) =>
-      (* the last block is frozen *)
-      f a' (l +ₗ last') cur_dist' true
-  | _ => None
-  end.
-
-
-(* Insert `it` into `stk` at `idx` unless `it` is equal to its neighbors. *)
-Definition item_insert_dedup (stk: stack) (new: item) (idx: nat) : stack :=
-  match idx with
-  | O =>
-    match stk with
-    | [] => [new]
-    | it' :: stk' => if decide (new = it') then stk else new :: stk
-    end
-  | S idx' =>
-    match stk !! idx', stk !! idx with
-    | None, None => take (S idx') stk ++ [new] ++ drop (S idx') stk
-    | Some it_l, Some it_r =>
-        if decide (new = it_l) then stk
-        else if decide (new = it_r) then stk
-             else take (S idx') stk ++ [new] ++ drop (S idx') stk
-    | Some it, None | None, Some it =>
-        if decide (new = it) then stk
-        else take (S idx') stk ++ [new] ++ drop (S idx') stk
-    end
-  end.
-
-(* Insert a `new` tag derived from a parent tag `derived_from`. *)
-Definition grant
-  (stk: stack) (derived_from: tag) (new: item) β : option stack :=
-  (* Figure out which access `new` allows *)
-  let access := if grants new.(perm) AccessWrite then AccessWrite else AccessRead in
-  (* Figure out which item grants our parent (`derived_from`) this kind of access *)
-  idx_p ← find_granting stk access derived_from;
-  match new.(perm) with
-  | SharedReadWrite =>
-    (* access is AccessWrite *)
-    new_idx ← find_first_write_incompatible (take idx_p.1 stk) idx_p.2;
-    Some (item_insert_dedup stk new new_idx)
-  | _ =>
-    (* an actual access check! *)
-    nstk' ← access1 stk access derived_from β;
-    Some (item_insert_dedup nstk'.2 new O)
-  end.
-
-Definition reborrowN α β l n old_tag new_tag pm prot :=
-  let it := mkItem pm new_tag prot in
-  for_each α l n false (λ stk, grant stk old_tag it β).
-
-(* This implements EvalContextPrivExt::reborrow *)
-(* TODO?: alloc.check_bounds(this, ptr, size)?; *)
-Definition reborrow h α β l (old_tag: tag) T (kind: ref_kind)
-  (new_tag: tag) (protector: option call_id) :=
-  match kind with
-  | SharedRef | RawRef false =>
-      (* for shared refs and const raw pointer, treat Unsafe as SharedReadWrite
-        and Freeze as SharedReadOnly *)
-      visit_freeze_sensitive h l T
-        (λ α' l' sz frozen,
-          (* If is in Unsafe, use SharedReadWrite, otherwise SharedReadOnly *)
-          let perm := if frozen then SharedReadOnly else SharedReadWrite in
-          reborrowN α' β l' sz old_tag new_tag perm protector) α
-  | UniqueRef false =>
-      (* mutable refs or Box use Unique *)
-      reborrowN α β l (tsize T) old_tag new_tag Unique protector
-  | UniqueRef true | RawRef true =>
-      (* mutable raw pointer uses SharedReadWrite *)
-      reborrowN α β l (tsize T) old_tag new_tag SharedReadWrite protector
-  end.
-
-(* Retag one pointer *)
-(* This implements EvalContextPrivExt::retag_reference *)
-Definition retag_ref h α β (clk: ptr_id) l (old_tag: tag) T
-  (kind: ref_kind) (protector: option call_id)
-  : option (tag * stacks * ptr_id) :=
-  match tsize T with
-  | O => (* Nothing to do for zero-sized types *)
-      Some (old_tag, α, clk)
-  | _ =>
-      let new_tag := match kind with
-                     | RawRef _ => Untagged
-                     | _ => Tagged clk
-                     end in
-      (* reborrow old_tag with new_tag *)
-      α' ← reborrow h α β l old_tag T kind new_tag protector;
-      Some (new_tag, α', S clk)
-  end.
-
-(* This implements EvalContextExt::retag *)
-Equations retag h α (clk: ptr_id) β (x: loc) (kind: retag_kind) T :
-  option (mem * stacks * ptr_id) :=
-  retag h α clk β x kind (Scalar _)         := Some (h, α, clk) ;
-  retag h α clk β x kind (Union _)          := Some (h, α, clk) ;
-  retag h α clk β x kind (Unsafe T)         := retag h α clk β x kind T ;
-  retag h α clk β x kind (Reference pk Tr) with h !! x :=
-  { | Some (LitV (LitLoc l otag)) :=
-        let qualify : option (ref_kind * option call_id) :=
-          match pk, kind with
-          (* Mutable reference *)
-          | RefPtr Mutable, _ =>
-              Some (UniqueRef (is_two_phase kind), adding_protector kind)
-          (* Immutable reference *)
-          | RefPtr Immutable, _ => Some (SharedRef, adding_protector kind)
-          (* If is both raw ptr and Raw retagging, no protector *)
-          | RawPtr mut, RawRt => Some (RawRef (bool_decide (mut = Mutable)), None)
-          (* Box pointer, no protector *)
-          | BoxPtr, _ => Some (UniqueRef false, None)
-          (* Ignore Raw pointer otherwise *)
-          | RawPtr _, _ => None
-          end in
-        match qualify with
-        | Some (rkind, protector) =>
-            bac ← retag_ref h α β clk l otag Tr rkind protector ;
-            Some (<[x := LitV (LitLoc l bac.1.1)]>h, bac.1.2, bac.2)
-        | None => Some (h, α, clk)
-        end ;
-    | _ := None } ;
-  retag h α clk β x kind (Product Ts)       := visit_LR h α clk x Ts
-    (* left-to-right visit to retag *)
-    where visit_LR h α (clk: ptr_id) (x: loc) (Ts: list type)
-      : option (mem * stacks * ptr_id) :=
-      { visit_LR h α clk x []         := Some (h, α, clk) ;
-        visit_LR h α clk x (T :: Ts)  :=
-          hac ← retag h α clk β x kind T ;
-          visit_LR hac.1.1 hac.1.2 hac.2 (x +ₗ (tsize T)) Ts } ;
-  retag h α clk β x kind (Sum Ts) with h !! x :=
-  { | Some (LitV (LitInt i)) :=
-        if decide (O ≤ i < length Ts)
-        then (* the discriminant is well-defined, visit with the
-                corresponding type *)
-          visit_lookup Ts (Z.to_nat i)
-        else None
-        where visit_lookup (Ts: list type) (i: nat) : option (mem * stacks * ptr_id) :=
-        { visit_lookup [] i             := None ;
-          visit_lookup (T :: Ts) O      := retag h α clk β (x +ₗ 1) kind T ;
-          visit_lookup (T :: Ts) (S i)  := visit_lookup Ts i } ;
-    | _ := None }
-  .
-
-Definition tag_value_included (tg: tag) (clk: ptr_id) : Prop :=
-  match tg with
-  | Tagged t => (t < clk)%nat
-  | _ => True
-  end.
-Infix "<b" := tag_value_included (at level 60, no associativity).
-Definition tag_values_included (vl: list immediate) clk :=
-  ∀ l tg, (LitV (LitLoc l tg)) ∈ vl → tg <b clk.
-Infix "<<b" := tag_values_included (at level 60, no associativity).
-
-(** Instrumented step for the stacked borrows *)
-(* This ignores CAS for now. *)
-Inductive instrumented_step h α β (clk: ptr_id):
-  event → mem → stacks → protectors → ptr_id → Prop :=
-| SilentIS :
-    instrumented_step h α β clk SilentEvt h α β clk
-(* | SysCallIS id :
-    instrumented_step h α β clk (SysCallEvt id) h α β clk *)
-(* This implements EvalContextExt::new_allocation. *)
-| AllocIS x T :
-    (* Tagged clk is the first borrow of the variable x,
-       used when accessing x directly (not through another pointer) *)
-    instrumented_step h α β clk
-                      (AllocEvt x (Tagged clk) T) h
-                      (init_stacks α x (tsize T) (Tagged clk)) β (S clk)
-(* This implements AllocationExtra::memory_read. *)
-| CopyIS α' l lbor T vl
-    (ACC: memory_read α β l lbor (tsize T) = Some α')
-    (BOR: vl <<b clk) :
-    instrumented_step h α β clk (CopyEvt l lbor T vl) h α' β clk
-(* This implements AllocationExtra::memory_written. *)
-| WriteIS α' l lbor T vl
-    (ACC: memory_written α β l lbor (tsize T) = Some α')
-    (BOR: vl <<b clk) :
-    instrumented_step h α β clk
-                      (WriteEvt l lbor T vl) h α' β clk
-(* This implements AllocationExtra::memory_deallocated. *)
-| DeallocIS α' l lbor T
-    (ACC: memory_deallocated α β l lbor (tsize T) = Some α') :
-    instrumented_step h α β clk
-                      (DeallocEvt l lbor T) h α' β clk
-| NewCallIS:
-    let call : call_id := fresh (dom (gset call_id) β) in
-    instrumented_step h α β clk
-                      (NewCallEvt call) h α (<[call := true]>β) clk
-| EndCallIS call
-    (ACTIVE: β !! call = Some true) :
-    instrumented_step h α β clk
-                      (EndCallEvt call) h α (<[call := false]>β) clk
-| RetagIS h' α' clk' x T kind
-    (FNBAR: match kind with FnEntry c => β !! c = Some true | _ => True end)
-    (RETAG: retag h α clk β x kind T = Some (h', α', clk')) :
-    instrumented_step h α β clk
-                      (RetagEvt x T kind) h' α' β clk'.
-
 (** COMBINED SEMANTICS -------------------------------------------------------*)
 Record state := mkState {
+  (* Global function table *)
+  cfns : fn_env;
+  (* Heap with base values *)
   cheap: mem;
+  (* Stacked borrows for the heap *)
   cstk : stacks;
+  (* Active call tracker *)
   cpro : protectors;
+  (* Counter for pointer tag generation *)
   cclk : ptr_id;
 }.
 
 Implicit Type (σ: state).
 
 Inductive head_step :
-  expr → state → list event → expr → state → list expr → Prop :=
+  expr → state → list mem_event → expr → state → list expr → Prop :=
   | HeadStep σ e e' efs ev h0 h' α' β' clock'
-      (BaseStep : base_step e σ.(cheap) ev e' h0 efs)
-      (InstrStep: instrumented_step h0 σ.(cstk) σ.(cpro) σ.(cclk) ev h' α' β' clock')
-  : head_step e σ [ev] e' (mkState h' α' β' clock') efs .
+      (ExprStep : expr_step σ.(cfns) e σ.(cheap) ev e' h0 efs)
+      (InstrStep: bor_step h0 σ.(cstk) σ.(cpro) σ.(cclk) ev h' α' β' clock')
+  : head_step e σ [ev] e' (mkState σ.(cfns) h' α' β' clock') efs .
 
 (** Closed expressions *)
-Lemma is_closed_weaken X Y e : is_closed X e → X ⊆ Y → is_closed Y e.
+(* Lemma is_closed_weaken X Y e : is_closed X e → X ⊆ Y → is_closed Y e.
 Proof.
   revert e X Y. fix FIX 1; destruct e=>X Y/=; try naive_solver.
   - rewrite !andb_True. intros [He Hel] HXY. split. by eauto.
     induction el=>/=; naive_solver.
-  - naive_solver set_solver.
   - intros Hel HXY. induction el=>/=; naive_solver.
+  - naive_solver set_solver.
   - rewrite !andb_True. intros [He Hel] HXY. split. by eauto.
     induction el=>/=; naive_solver.
 Qed.
 
 Lemma is_closed_weaken_nil X e : is_closed [] e → is_closed X e.
-Proof. intros. by apply is_closed_weaken with [], list_subseteq_nil. Qed.
+Proof. intros. by apply is_closed_weaken with [], list_subseteq_nil. Qed. *)
 
 Lemma is_closed_subst X e x es : is_closed X e → x ∉ X → subst x es e = e.
 Proof.
@@ -1068,64 +60,53 @@ Proof. intros. apply is_closed_subst with []; set_solver. Qed.
 
 Lemma is_closed_of_val X v : is_closed X (of_val v).
 Proof.
-  apply is_closed_weaken_nil. destruct v as [[]|vl|]; auto.
+  destruct v as [[]|vl|]; auto.
   induction vl as [|v vl]; first auto. destruct v; simpl; auto.
 Qed.
 
-Lemma to_immediates_cons vl e el:
-  to_immediates vl (e :: el) = v ← to_immediate e; to_immediates (vl ++ [v]) el.
+Lemma to_lits_cons vl e el:
+  to_lits vl (e :: el) = v ← to_lit e; to_lits (vl ++ [v]) el.
 Proof.
-  rewrite /to_immediates /=. destruct (to_immediate e); simpl; [done|].
+  rewrite /to_lits /=. destruct (to_lit e); simpl; [done|].
   by induction el.
 Qed.
-Lemma to_immediates_app vl el1 el2 :
-  to_immediates vl (el1 ++ el2) = vl' ← to_immediates vl el1; to_immediates vl' el2.
+Lemma to_lits_app vl el1 el2 :
+  to_lits vl (el1 ++ el2) = vl' ← to_lits vl el1; to_lits vl' el2.
 Proof.
   revert vl. induction el1 as [|e el1 IH]; intros vl; [done|].
-  rewrite /= 2!to_immediates_cons option_bind_assoc.
+  rewrite /= 2!to_lits_cons option_bind_assoc.
   apply option_bind_ext; [|done]. intros; by apply IH.
 Qed.
 
-Lemma to_of_immediate v: to_immediate (of_immediate v) = Some v.
-Proof.
-  destruct v; [done|]. simplify_option_eq; [|done].
-  repeat f_equal. apply (proof_irrel _).
-Qed.
-Lemma of_to_immediate e v : to_immediate e = Some v → of_immediate v = e.
-Proof. destruct e=>//=; [|case decide => ? //]; by intros [= <-]. Qed.
-Lemma to_of_immediates vl1 vl2 :
-  to_immediates vl1 (of_immediate <$> vl2) = Some (vl1 ++ vl2).
+Lemma to_of_lits vl1 vl2 :
+  to_lits vl1 (Lit <$> vl2) = Some (vl1 ++ vl2).
 Proof.
   revert vl1. induction vl2 as [|v vl2 IH]; intros vl1; [by rewrite app_nil_r|].
-  rewrite fmap_cons to_immediates_cons to_of_immediate /= IH. f_equal.
+  rewrite fmap_cons to_lits_cons  /= IH. f_equal.
   by rewrite (cons_middle v vl1 vl2) app_assoc.
 Qed.
-Lemma of_to_immediates vl1 el2 vl:
-  to_immediates vl1 el2 = Some vl →
-  of_val (TValV vl) = (TVal ((of_immediate <$> vl1) ++ el2)).
+
+Lemma of_to_lit e v : to_lit e = Some v → Lit v = e.
+Proof. destruct e=>//= Eq. by inversion Eq. Qed.
+Lemma of_to_lits vl1 el2 vl:
+  to_lits vl1 el2 = Some vl →
+  of_val (TValV vl) = (TVal ((Lit <$> vl1) ++ el2)).
 Proof.
   revert vl1 vl. induction el2 as [|e el2 IH]; intros vl1 vl.
-  - by rewrite /to_immediates /= app_nil_r => [[->]].
-  - rewrite to_immediates_cons.
-    destruct (to_immediate e) as [v|] eqn:Eqv; [|done].
+  - by rewrite /to_lits /= app_nil_r => [[->]].
+  - rewrite to_lits_cons.
+    destruct (to_lit e) as [v|] eqn:Eqv; [|done].
     move => /(IH _ _) ->. f_equal.
-    by rewrite fmap_app -(of_to_immediate _ _ Eqv) /= -app_assoc cons_middle.
+    by rewrite fmap_app -(of_to_lit _ _ Eqv) /= -app_assoc cons_middle.
 Qed.
-Instance of_immediate_inj : Inj (=) (=) of_immediate.
-Proof. by intros ?? Hv; apply (inj Some); rewrite -2!to_of_immediate Hv /=. Qed.
 
 Lemma to_of_val v : to_val (of_val v) = Some v.
-Proof.
-  destruct v as [[]|vl|]; [done|..|done].
-  - simplify_option_eq; [|done]. repeat f_equal. apply (proof_irrel _).
-  - by rewrite /= to_of_immediates /=.
-Qed.
+Proof. destruct v as [[]|vl|]; auto. by rewrite /= to_of_lits. Qed.
 Lemma of_to_val e v : to_val e = Some v → of_val v = e.
 Proof.
-  destruct e=>//=; [|case decide => ? //
-                    |destruct (to_immediates [] el) as [vl|] eqn:Eq; [|done]
+  destruct e=>//=; [|destruct (to_lits [] el) as [vl|] eqn:Eq; [|done]
                     |]; intros [= <-]; auto.
-  by rewrite (of_to_immediates _ _ _ Eq).
+  by rewrite (of_to_lits _ _ _ Eq).
 Qed.
 
 Instance of_val_inj : Inj (=) (=) of_val.
@@ -1134,14 +115,14 @@ Proof. by intros ?? Hv; apply (inj Some); rewrite -2!to_of_val Hv /=. Qed.
 Lemma is_closed_to_val X e v : to_val e = Some v → is_closed X e.
 Proof. intros <-%of_to_val. apply is_closed_of_val. Qed.
 
-Lemma subst_is_closed X x es e :
+(* Lemma subst_is_closed X x es e :
   is_closed X es → is_closed (x::X) e → is_closed X (subst x es e).
 Proof.
   revert e X. fix FIX 1; destruct e=>X //=; repeat (case_bool_decide=>//=);
     try naive_solver; rewrite ?andb_True; intros.
   - set_solver.
   - split; first naive_solver. induction el; naive_solver.
-  - eauto using is_closed_weaken with set_solver.
+  - (* eauto using is_closed_weaken with set_solver. *)
   - eapply is_closed_weaken; first done.
     destruct (decide (BNamed x = f)), (decide (BNamed x ∈ xl)); set_solver.
   - induction el; naive_solver.
@@ -1151,6 +132,7 @@ Qed.
 Lemma subst'_is_closed X b es e :
   is_closed X es → is_closed (b:b:X) e → is_closed X (subst' b es e).
 Proof. destruct b; first done. apply subst_is_closed. Qed.
+ *)
 
 (** Equality and other typeclass stuff *)
 
@@ -1171,14 +153,18 @@ Instance lit_countable : Countable lit.
 Proof.
   refine (inj_countable
           (λ v, match v with
-              | LitPoison => inl ()
-              | LitLoc l bor => inr (inl (l,bor))
-              | LitInt n => inr (inr n)
+              | LitPoison => inl (inl (inl ()))
+              | LitLoc l bor => inl (inl (inr (l,bor)))
+              | LitInt n => inl (inr (inl n))
+              | LitFnPtr n => inl (inr (inr n))
+              | LitCall n => inr n
               end)
           (λ s, match s with
-              | inl () => Some LitPoison
-              | inr (inl (l,bor)) => Some $ LitLoc l bor
-              | inr (inr n) => Some $ LitInt n
+              | inl (inl (inl ())) => Some LitPoison
+              | inl (inl (inr (l,bor))) => Some $ LitLoc l bor
+              | inl (inr (inl n)) => Some $ LitInt n
+              | inl (inr (inr n)) => Some $ LitFnPtr n
+              | inr n => Some $ LitCall n
               end) _); by intros [].
 Qed.
 
@@ -1394,13 +380,13 @@ Canonical Structure stateC := leibnizC state.
 Instance fill_item_inj Ki : Inj (=) (=) (fill_item Ki).
 Proof. destruct Ki; intros ???; simplify_eq/=; auto with f_equal. Qed.
 
-Lemma to_immediates_elem_Some vl vl' el e:
-  to_immediates vl el = Some vl' → e ∈ el → is_Some (to_val e).
+Lemma to_lits_elem_Some vl vl' el e:
+  to_lits vl el = Some vl' → e ∈ el → is_Some (to_val e).
 Proof.
   revert vl. induction el as [|e' ? IH]; intros vl; [by intros _ ?%elem_of_nil|].
-  rewrite to_immediates_cons.
-  destruct (to_immediate e') as [v'|] eqn:Eq'; [|done].
-  move => /= /IH In /elem_of_cons [->|/In //]. rewrite -(of_to_immediate _ _ Eq').
+  rewrite to_lits_cons.
+  destruct (to_lit e') as [v'|] eqn:Eq'; [|done].
+  move => /= /IH In /elem_of_cons [->|/In //]. rewrite -(of_to_lit _ _ Eq').
   destruct v'; simpl; [|rewrite decide_left]; naive_solver.
 Qed.
 
@@ -1408,19 +394,19 @@ Lemma fill_item_val Ki e :
   is_Some (to_val (fill_item Ki e)) → is_Some (to_val e).
 Proof.
   intros [v ?]. destruct Ki; simplify_option_eq; eauto.
-  eapply to_immediates_elem_Some; eauto. set_solver.
+  eapply to_lits_elem_Some; eauto. set_solver.
 Qed.
 
-Lemma to_immediates_elem_None vl el e:
-  to_val e = None → e ∈ el → to_immediates vl el = None.
+Lemma to_lits_elem_None vl el e:
+  to_val e = None → e ∈ el → to_lits vl el = None.
 Proof.
   revert vl. induction el as [|e' ? IH]; intros vl; [by intros _ ?%elem_of_nil|].
-  rewrite to_immediates_cons.
-  destruct (to_immediate e') as [v'|] eqn:Eq'; [|done].
+  rewrite to_lits_cons.
+  destruct (to_lit e') as [v'|] eqn:Eq'; [|done].
   move => /= EqN /elem_of_cons [?|IN].
   - subst. exfalso.
-    move : Eq' EqN. rewrite /to_immediate /to_val.
-    destruct e'; simplify_eq; try done. rewrite /to_immediate /=.
+    move : Eq' EqN. rewrite /to_lit /to_val.
+    destruct e'; simplify_eq; try done. rewrite /to_lit /=.
     case decide; try done.
   - by apply IH.
 Qed.
@@ -1429,7 +415,7 @@ Lemma fill_item_no_val Ki e :
   to_val e = None → to_val (fill_item Ki e) = None.
 Proof.
   intros EqN. destruct Ki; simplify_option_eq; eauto.
-  rewrite (to_immediates_elem_None _ _ e EqN) // elem_of_app.
+  rewrite (to_lits_elem_None _ _ e EqN) // elem_of_app.
   by right; left.
 Qed.
 
@@ -1475,41 +461,8 @@ Proof.
   split; apply _ || eauto using to_of_val, of_to_val, val_head_stuck,
     fill_item_val, fill_item_no_val_inj, head_ctx_step_val.
 Qed.
-End bor_lang.
 
 (** Language *)
 Canonical Structure bor_ectxi_lang := EctxiLanguage bor_lang.bor_lang_mixin.
 Canonical Structure bor_ectx_lang := EctxLanguageOfEctxi bor_ectxi_lang.
 Canonical Structure bor_lang := LanguageOfEctx bor_ectx_lang.
-
-Export bor_lang.
-
-(** Some derived forms. *)
-Notation Lam xl e := (Rec BAnon xl e).
-Notation Let x e1 e2 := (App (Lam [x] e2) [e1]).
-Notation Seq e1 e2 := (Let BAnon e1 e2).
-Notation LamV xl e := (ImmV (RecV BAnon xl e)).
-Notation LetCtx x e2 := (AppRCtx (LamV [x] e2) [] []).
-Notation SeqCtx e2 := (LetCtx BAnon e2).
-Notation Skip := (Seq (Lit LitPoison) (Lit LitPoison)).
-Notation If e0 e1 e2 := (Case e0 [e2;e1]).
-
-Coercion lit_of_bool : bool >-> lit.
-Coercion LitInt : Z >-> lit.
-
-(** Shifting for locations *)
-Lemma shift_loc_assoc l n n' : l +ₗ n +ₗ n' = l +ₗ (n + n').
-Proof. rewrite /shift_loc /=. f_equal. lia. Qed.
-Lemma shift_loc_0 l : l +ₗ 0 = l.
-Proof. destruct l as [b o]. rewrite /shift_loc /=. f_equal. lia. Qed.
-
-Lemma shift_loc_assoc_nat l (n n' : nat) : l +ₗ n +ₗ n' = l +ₗ (n + n')%nat.
-Proof. rewrite /shift_loc /=. f_equal. lia. Qed.
-Lemma shift_loc_0_nat l : l +ₗ 0%nat = l.
-Proof. destruct l as [b o]. rewrite /shift_loc /=. f_equal. lia. Qed.
-
-Instance shift_loc_inj l : Inj (=) (=) (shift_loc l).
-Proof. destruct l as [b o]; intros n n' [=?]; lia. Qed.
-
-Lemma shift_loc_block l n : (l +ₗ n).1 = l.1.
-Proof. done. Qed.
