theories/bor_semantics.v
@@ -1,0 +1,453 @@
+From Equations Require Import Equations.
+From stdpp Require Export gmap.
+
+From stbor Require Export lang_base notation.
+
+Set Default Proof Using "Type".
+
+(*** STACKED BORROWS SEMANTICS ---------------------------------------------***)
+
+Implicit Type (α: stacks) (β: protectors) (t: ptr_id) (c: call_id) (T: type).
+
+(** CORE SEMANTICS *)
+
+Inductive access_kind := AccessRead | AccessWrite.
+
+Definition grants (perm: permission) (access: access_kind) : bool :=
+  match perm, access with
+  | Disabled, _ => false
+  (* All items grant read access.
+    All items except SharedReadOnly grant write access. *)
+  | SharedReadOnly, AccessWrite => false
+  | _, _ => true
+  end.
+
+Definition matched_grant (access: access_kind) (bor: tag) (it: item) :=
+  grants it.(perm) access ∧ it.(tg) = bor.
+Instance matched_grant_dec (access: access_kind) (bor: tag) :
+  Decision (matched_grant access bor it) := _.
+
+(* This is different from Miri's implementation: left-to-right is top-to-bottom
+  of the stack. So 0 is top of the stack. The index returned by this function
+  also follows this scheme (smaller means higher in the stack). *)
+Definition find_granting (stk: stack) (access: access_kind) (bor: tag) :
+  option (nat * permission) :=
+  (λ nit, (nit.1, nit.2.(perm))) <$> (list_find (matched_grant access bor) stk).
+
+Definition is_active β (c: call_id) : bool :=
+  bool_decide (β !! c = Some true).
+Definition is_active_protector β (it: item) :=
+  match it.(protector) with
+  | Some c => β !! c = Some true
+  | _ => False
+  end.
+Instance is_active_protector_dec β : Decision (is_active_protector β it).
+Proof. intros it. rewrite /is_active_protector. case_match; solve_decision. Qed.
+
+(* Find the top active protector *)
+Definition find_top_active_protector β (stk: stack) :=
+  list_find (is_active_protector β) stk.
+
+(* Checks to deallocate a location: Like a write access, but also there must be
+  no active protectors at all. *)
+Definition dealloc1 (stk: stack) (bor: tag) β : option unit :=
+  (* Step 1: Find granting item. *)
+  found ← find_granting stk AccessWrite bor;
+  (* Step 2: Check that there are no active protectors left. *)
+  if find_top_active_protector β stk then None else Some ().
+
+(* Find the index RIGHT BEFORE the first incompatiable item *)
+Definition find_first_write_incompatible
+  (stk: stack) (pm: permission) : option nat :=
+  match pm with
+  | Unique => Some (length stk)
+  | SharedReadWrite =>
+      match (list_find (λ it, it.(perm) ≠ SharedReadWrite) (reverse stk)) with
+      | Some (idx, _) => Some ((length stk) - idx)%nat
+      | _ => Some O
+      end
+  | SharedReadOnly | Disabled => None
+  end.
+
+Definition check_protector β (it: item) : bool :=
+  match it.(protector) with
+  | None => true
+  | Some c => if is_active β c then false else true
+  end.
+
+(* Remove from `stk` the items before `idx`.
+  Check that removed items do not have active protectors.
+  The check is run from the top to before the `idx`. *)
+Fixpoint remove_check β (stk: stack) (idx: nat) : option stack :=
+  match idx, stk with
+  (* Assumption: idx ≤ length stk *)
+  | S _, [] => None
+  | O, stk => Some stk
+  | S idx, it :: stk =>
+      if check_protector β it then remove_check β stk idx else None
+  end.
+
+(* Replace any Unique permission with Disabled, starting from the top of the
+  stack. Check that replaced item do not have active protectors *)
+Fixpoint replace_check' β (acc stk : stack) : option stack :=
+  match stk with
+  | [] => Some acc
+  | it :: stk =>
+      if decide (it.(perm) = Unique) then
+        if check_protector β it
+        then let new := mkItem Disabled it.(tg) it.(protector) in
+             replace_check' β (acc ++ [new]) stk
+        else None
+      else replace_check' β (acc ++ [it]) stk
+  end.
+Definition replace_check β (stk: stack) : option stack :=
+  replace_check' β [] stk.
+
+(* Test if a memory `access` using pointer tagged `tg` is granted.
+   If yes, return the index (in the old stack) of the item that granted it,
+   as well as the new stack. *)
+Definition access1 (stk: stack) (access: access_kind) (tg: tag) β
+  : option (nat * stack) :=
+  (* Step 1: Find granting item. *)
+  idx_p ← find_granting stk access tg;
+  (* Step 2: Remove incompatiable items. *)
+  match access with
+  | AccessWrite =>
+      (* Remove everything above the write-compatible items, like a proper stack. *)
+      incompat_idx ← find_first_write_incompatible (take idx_p.1 stk) idx_p.2;
+      stk' ← remove_check β (take idx_p.1 stk) incompat_idx;
+      Some (idx_p.1, stk' ++ drop idx_p.1 stk)
+  | AccessRead =>
+      (* On a read, *disable* all `Unique` above the granting item. *)
+      stk' ← replace_check β (take idx_p.1 stk);
+      Some (idx_p.1, stk' ++ drop idx_p.1 stk)
+  end.
+
+(* Initialize [l, l + n) with singleton stacks of `tg` *)
+Fixpoint init_stacks α (l:loc) (n:nat) (tg: tag) : stacks :=
+  match n with
+  | O => α
+  | S n => <[l:= [mkItem Unique tg None]]>(init_stacks α (l +ₗ 1) n tg)
+  end.
+
+Fixpoint for_each α (l:loc) (n:nat) (dealloc: bool) (f: stack → option stack)
+  : option stacks :=
+  match n with
+  | O => Some α
+  | S n =>
+      let l' := (l +ₗ n) in
+      stk ← α !! l'; stk' ← f stk ;
+      if dealloc
+      then for_each (delete l' α) l n dealloc f
+      else for_each (<[l':=stk']> α) l n dealloc f
+  end.
+
+(* Perform the access check on a block of continuous memory.
+ * This implements Stacks::memory_read/memory_written/memory_deallocated. *)
+Definition memory_read α β l (tg: tag) (n: nat) : option stacks :=
+  for_each α l n false (λ stk, nstk' ← access1 stk AccessRead tg β; Some nstk'.2).
+Definition memory_written α β l (tg: tag) (n: nat) : option stacks :=
+  for_each α l n false (λ stk, nstk' ← access1 stk AccessWrite tg β; Some nstk'.2).
+Definition memory_deallocated α β l (tg: tag) (n: nat) : option stacks :=
+  for_each α l n true (λ stk, dealloc1 stk tg β ;; Some []).
+
+Definition unsafe_action
+  {A: Type} (f: A → loc → nat → bool → option A) (a: A) (l: loc)
+  (last frozen_size unsafe_size: nat) :
+  option (A * (nat * nat)) :=
+  (* Anything between the last UnsafeCell and this UnsafeCell is frozen *)
+  a' ← f a (l +ₗ last) frozen_size true;
+  (* This UnsafeCell is not frozen *)
+  let cur_off := (last + frozen_size)%nat in
+    a'' ← f a' (l +ₗ cur_off) unsafe_size false ;
+    Some (a'', ((cur_off + unsafe_size)%nat, O))
+  .
+
+(** Reborrow *)
+
+(* visit the type left-to-right and apply the action `f`.
+ + `last` is the offset of `l` from the last UnsafeCell,
+ + `cur_dist` is the distance between `last` and the current offset of the
+   visit, which is also the start of the sub-type `T`.
+ + a` of type A is the accumulator for the visit.
+ When an UnsafeCell is found, the action `f` is applied twice, through
+ `unsafe_action`:
+ - First `f` is applied for the frozen block, which is the range
+   [last, last + cur_dist). `f` is applied with the boolean flag `true`
+   (for frozen).
+ - Then `f` is applied for the unfrozen block, which is the range
+   [last + cur_dist, last + cur_dist + unsafe_block_size). `f` is applied with
+   the boolean flag `false`. *)
+Section blah.
+Context {A: Type}.
+Equations visit_freeze_sensitive'
+  (h: mem) (l: loc) (f: A → loc → nat → bool → option A)
+  (a: A) (last cur_dist: nat) (T: type) : option (A * (nat * nat)) :=
+  visit_freeze_sensitive' h l f a last cur_dist (Scalar n) :=
+    (* consider frozen, simply extend the distant by n *)
+      Some (a, (last, cur_dist + n)%nat) ;
+  visit_freeze_sensitive' h l f a last cur_dist (Reference _ _) :=
+    (* consider frozen, extend the distant by 1 *)
+      Some (a, (last, S cur_dist)) ;
+  visit_freeze_sensitive' h l f a last cur_dist (Unsafe T) :=
+    (* reach an UnsafeCell, apply the action `f` and return new `last` and
+        `cur_dist` *)
+      unsafe_action f a l last cur_dist (tsize T) ;
+  visit_freeze_sensitive' h l f a last cur_dist (Union Ts) :=
+    (* If it's a union, look at the type to see if there is UnsafeCell *)
+      if is_freeze (Union Ts)
+      (* No UnsafeCell, consider the whole block frozen and simply extend the
+          distant. *)
+      then Some (a, (last, cur_dist + (tsize (Union Ts)))%nat)
+      (* There can be UnsafeCell, consider the whole block unfrozen and perform
+          `f a _ _ false` on the whole block. `unsafe_action` will return the
+          offsets for the following visit. *)
+      else unsafe_action f a l last cur_dist (tsize (Union Ts)) ;
+  visit_freeze_sensitive' h l f a last cur_dist (Product Ts) :=
+    (* Try a shortcut *)
+      if is_freeze (Product Ts)
+      (* No UnsafeCell, consider the whole block frozen and simply extend the
+        distant. *)
+      then Some (a, (last, cur_dist + (tsize (Product Ts)))%nat)
+      (* This implements left-to-right search on the type, which guarantees
+        that the offsets are increasing. *)
+      else visit_LR a last cur_dist Ts
+        where visit_LR (a: A) (last cur_dist: nat) (Ts: list type)
+          : option (A * (nat * nat)) :=
+          { visit_LR a last cur_dist [] := Some (a, (last, cur_dist)) ;
+            visit_LR a last cur_dist (T :: Ts) :=
+              alc ← visit_freeze_sensitive' h l f a last cur_dist T ;
+              visit_LR alc.1 alc.2.1 alc.2.2 Ts } ;
+  visit_freeze_sensitive' h l f a last cur_dist (Sum Ts) :=
+    (* Try a shortcut *)
+      if is_freeze (Sum Ts)
+      (* No UnsafeCell, consider the whole block frozen and simply extend the
+          distant. *)
+      then Some (a, (last, cur_dist + (tsize (Sum Ts)))%nat)
+      else
+        match h !! (l +ₗ (last + cur_dist)) with
+        (* This looks up the current state to see which discriminant currently
+            is active (which is an integer) and redirect the visit for the type
+            of that discriminant. Note that this consitutes a read-access, and
+            should adhere to the access checks. But we are skipping them here.
+            FIXME *)
+        | Some (LitInt i) =>
+            if decide (O ≤ i)
+            then (* the discriminant is well-defined, visit with the
+                    corresponding type *)
+              alc ← visit_lookup Ts (Z.to_nat i) ;
+              (* Anything in the padding is considered frozen and will be
+                 applied with the action by the following visit.
+                 `should_offset` presents the offset that the visit SHOULD
+                 arrive at after the visit. If there are padding bytes left,
+                 they will be added to the cur_dist. *)
+              let should_offset := (last + cur_dist + tsize (Sum Ts))%nat in
+                Some (alc.1, (alc.2.1, (should_offset - alc.2.1)%nat))
+            else None
+        | _ => None
+        end
+      where visit_lookup (Ts: list type) (i: nat) : option (A * (nat * nat)) :=
+            { visit_lookup [] _             := None ;
+              visit_lookup (T :: _) O      :=
+                visit_freeze_sensitive' h l f a last (S cur_dist) T ;
+              visit_lookup (T :: Ts) (S i)  := visit_lookup Ts i }
+  .
+End blah.
+
+Definition visit_freeze_sensitive {A: Type}
+  h (l: loc) (T: type) (f: A → loc → nat → bool → option A) (a: A) : option A :=
+  match visit_freeze_sensitive' h l f a O O T with
+  | Some (a', (last', cur_dist')) =>
+      (* the last block is frozen *)
+      f a' (l +ₗ last') cur_dist' true
+  | _ => None
+  end.
+
+
+(* Insert `it` into `stk` at `idx` unless `it` is equal to its neighbors. *)
+Definition item_insert_dedup (stk: stack) (new: item) (idx: nat) : stack :=
+  match idx with
+  | O =>
+    match stk with
+    | [] => [new]
+    | it' :: stk' => if decide (new = it') then stk else new :: stk
+    end
+  | S idx' =>
+    match stk !! idx', stk !! idx with
+    | None, None => take (S idx') stk ++ [new] ++ drop (S idx') stk
+    | Some it_l, Some it_r =>
+        if decide (new = it_l) then stk
+        else if decide (new = it_r) then stk
+             else take (S idx') stk ++ [new] ++ drop (S idx') stk
+    | Some it, None | None, Some it =>
+        if decide (new = it) then stk
+        else take (S idx') stk ++ [new] ++ drop (S idx') stk
+    end
+  end.
+
+(* Insert a `new` tag derived from a parent tag `derived_from`. *)
+Definition grant
+  (stk: stack) (derived_from: tag) (new: item) β : option stack :=
+  (* Figure out which access `new` allows *)
+  let access := if grants new.(perm) AccessWrite then AccessWrite else AccessRead in
+  (* Figure out which item grants our parent (`derived_from`) this kind of access *)
+  idx_p ← find_granting stk access derived_from;
+  match new.(perm) with
+  | SharedReadWrite =>
+    (* access is AccessWrite *)
+    new_idx ← find_first_write_incompatible (take idx_p.1 stk) idx_p.2;
+    Some (item_insert_dedup stk new new_idx)
+  | _ =>
+    (* an actual access check! *)
+    nstk' ← access1 stk access derived_from β;
+    Some (item_insert_dedup nstk'.2 new O)
+  end.
+
+Definition reborrowN α β l n old_tag new_tag pm prot :=
+  let it := mkItem pm new_tag prot in
+  for_each α l n false (λ stk, grant stk old_tag it β).
+
+(* This implements EvalContextPrivExt::reborrow *)
+(* TODO?: alloc.check_bounds(this, ptr, size)?; *)
+Definition reborrow h α β l (old_tag: tag) T (kind: ref_kind)
+  (new_tag: tag) (protector: option call_id) :=
+  match kind with
+  | SharedRef | RawRef false =>
+      (* for shared refs and const raw pointer, treat Unsafe as SharedReadWrite
+        and Freeze as SharedReadOnly *)
+      visit_freeze_sensitive h l T
+        (λ α' l' sz frozen,
+          (* If is in Unsafe, use SharedReadWrite, otherwise SharedReadOnly *)
+          let perm := if frozen then SharedReadOnly else SharedReadWrite in
+          reborrowN α' β l' sz old_tag new_tag perm protector) α
+  | UniqueRef false =>
+      (* mutable refs or Box use Unique *)
+      reborrowN α β l (tsize T) old_tag new_tag Unique protector
+  | UniqueRef true | RawRef true =>
+      (* mutable raw pointer uses SharedReadWrite *)
+      reborrowN α β l (tsize T) old_tag new_tag SharedReadWrite protector
+  end.
+
+(* Retag one pointer *)
+(* This implements EvalContextPrivExt::retag_reference *)
+Definition retag_ref h α β (clk: ptr_id) l (old_tag: tag) T
+  (kind: ref_kind) (protector: option call_id)
+  : option (tag * stacks * ptr_id) :=
+  match tsize T with
+  | O => (* Nothing to do for zero-sized types *)
+      Some (old_tag, α, clk)
+  | _ =>
+      let new_tag := match kind with
+                     | RawRef _ => Untagged
+                     | _ => Tagged clk
+                     end in
+      (* reborrow old_tag with new_tag *)
+      α' ← reborrow h α β l old_tag T kind new_tag protector;
+      Some (new_tag, α', S clk)
+  end.
+
+(* This implements EvalContextExt::retag *)
+Equations retag (h: mem) α (clk: ptr_id) β (x: loc) (kind: retag_kind) T :
+  option (mem * stacks * ptr_id) :=
+  retag h α clk β x kind (Scalar _)         := Some (h, α, clk) ;
+  retag h α clk β x kind (Union _)          := Some (h, α, clk) ;
+  retag h α clk β x kind (Unsafe T)         := retag h α clk β x kind T ;
+  retag h α clk β x kind (Reference pk Tr) with h !! x :=
+  { | Some (LitLoc l otag) :=
+        let qualify : option (ref_kind * option call_id) :=
+          match pk, kind with
+          (* Mutable reference *)
+          | RefPtr Mutable, _ =>
+              Some (UniqueRef (is_two_phase kind), adding_protector kind)
+          (* Immutable reference *)
+          | RefPtr Immutable, _ => Some (SharedRef, adding_protector kind)
+          (* If is both raw ptr and Raw retagging, no protector *)
+          | RawPtr mut, RawRt => Some (RawRef (bool_decide (mut = Mutable)), None)
+          (* Box pointer, no protector *)
+          | BoxPtr, _ => Some (UniqueRef false, None)
+          (* Ignore Raw pointer otherwise *)
+          | RawPtr _, _ => None
+          end in
+        match qualify with
+        | Some (rkind, protector) =>
+            bac ← retag_ref h α β clk l otag Tr rkind protector ;
+            Some (<[x := LitLoc l bac.1.1]>h, bac.1.2, bac.2)
+        | None => Some (h, α, clk)
+        end ;
+    | _ := None } ;
+  retag h α clk β x kind (Product Ts)       := visit_LR h α clk x Ts
+    (* left-to-right visit to retag *)
+    where visit_LR h α (clk: ptr_id) (x: loc) (Ts: list type)
+      : option (mem * stacks * ptr_id) :=
+      { visit_LR h α clk x []         := Some (h, α, clk) ;
+        visit_LR h α clk x (T :: Ts)  :=
+          hac ← retag h α clk β x kind T ;
+          visit_LR hac.1.1 hac.1.2 hac.2 (x +ₗ (tsize T)) Ts } ;
+  retag h α clk β x kind (Sum Ts) with h !! x :=
+  { | Some (LitInt i) :=
+        if decide (O ≤ i < length Ts)
+        then (* the discriminant is well-defined, visit with the
+                corresponding type *)
+          visit_lookup Ts (Z.to_nat i)
+        else None
+        where visit_lookup (Ts: list type) (i: nat) : option (mem * stacks * ptr_id) :=
+        { visit_lookup [] i             := None ;
+          visit_lookup (T :: Ts) O      := retag h α clk β (x +ₗ 1) kind T ;
+          visit_lookup (T :: Ts) (S i)  := visit_lookup Ts i } ;
+    | _ := None }
+  .
+
+Definition tag_value_included (tg: tag) (clk: ptr_id) : Prop :=
+  match tg with
+  | Tagged t => (t < clk)%nat
+  | _ => True
+  end.
+Infix "<b" := tag_value_included (at level 60, no associativity).
+Definition tag_values_included (vl: list lit) clk :=
+  ∀ l tg, LitLoc l tg ∈ vl → tg <b clk.
+Infix "<<b" := tag_values_included (at level 60, no associativity).
+
+(** Instrumented step for the stacked borrows *)
+(* This ignores CAS for now. *)
+Inductive bor_step h α β (clk: ptr_id):
+  mem_event → mem → stacks → protectors → ptr_id → Prop :=
+| SilentIS :
+    bor_step h α β clk SilentEvt h α β clk
+(* | SysCallIS id :
+    bor_step h α β clk (SysCallEvt id) h α β clk *)
+(* This implements EvalContextExt::new_allocation. *)
+| AllocIS x T :
+    (* Tagged clk is the first borrow of the variable x,
+       used when accessing x directly (not through another pointer) *)
+    bor_step h α β clk
+                      (AllocEvt x (Tagged clk) T) h
+                      (init_stacks α x (tsize T) (Tagged clk)) β (S clk)
+(* This implements AllocationExtra::memory_read. *)
+| CopyIS α' l lbor T vl
+    (ACC: memory_read α β l lbor (tsize T) = Some α')
+    (BOR: vl <<b clk) :
+    bor_step h α β clk (CopyEvt l lbor T vl) h α' β clk
+(* This implements AllocationExtra::memory_written. *)
+| WriteIS α' l lbor T vl
+    (ACC: memory_written α β l lbor (tsize T) = Some α')
+    (BOR: vl <<b clk) :
+    bor_step h α β clk
+                      (WriteEvt l lbor T vl) h α' β clk
+(* This implements AllocationExtra::memory_deallocated. *)
+| DeallocIS α' l lbor T
+    (ACC: memory_deallocated α β l lbor (tsize T) = Some α') :
+    bor_step h α β clk
+                      (DeallocEvt l lbor T) h α' β clk
+| NewCallIS name:
+    let call : call_id := fresh (dom (gset call_id) β) in
+    bor_step h α β clk
+                      (NewCallEvt name call) h α (<[call := true]>β) clk
+| EndCallIS call
+    (ACTIVE: β !! call = Some true) :
+    bor_step h α β clk
+                      (EndCallEvt call) h α (<[call := false]>β) clk
+| RetagIS h' α' clk' x T kind
+    (FNBAR: match kind with FnEntry c => β !! c = Some true | _ => True end)
+    (RETAG: retag h α clk β x kind T = Some (h', α', clk')) :
+    bor_step h α β clk
+                      (RetagEvt x T kind) h' α' β clk'.
