theories/expr_semantics.v
@@ -1,0 +1,328 @@
+From Equations Require Import Equations.
+From stdpp Require Export gmap.
+
+From stbor Require Export lang_base notation.
+
+Set Default Proof Using "Type".
+
+(*** EXPRESSION SEMANTICS --------------------------------------------------***)
+
+(** Substitution *)
+Fixpoint subst (x : string) (es : expr) (e : expr) : expr :=
+  match e with
+  | Var y => if bool_decide (y = x) then es else Var y
+  | Lit l => Lit l
+  (* | Rec f xl e =>
+    Rec f xl $ if bool_decide (BNamed x ≠ f ∧ BNamed x ∉ xl) then subst x es e else e *)
+  | Call e el => Call (subst x es e) (map (subst x es) el)
+  | EndCall e => EndCall (subst x es e)
+  | Place l tag T => Place l tag T
+  (* | App e1 el => App (subst x es e1) (map (subst x es) el) *)
+  | BinOp op e1 e2 => BinOp op (subst x es e1) (subst x es e2)
+  | TVal el => TVal (map (subst x es) el)
+  | Proj e1 e2 => Proj (subst x es e1) (subst x es e2)
+  | Conc e1 e2 => Conc (subst x es e1) (subst x es e2)
+  | Copy e => Copy (subst x es e)
+  | Write e1 e2 => Write (subst x es e1) (subst x es e2)
+  | Alloc T => Alloc T
+  | Free e => Free (subst x es e)
+  (* | CAS e0 e1 e2 => CAS (subst x es e0) (subst x es e1) (subst x es e2) *)
+  (* | AtomWrite e1 e2 => AtomWrite (subst x es e1) (subst x es e2) *)
+  (* | AtomRead e => AtomRead (subst x es e) *)
+  | Deref e T => Deref (subst x es e) T
+  | Ref e => Ref (subst x es e)
+  | Field e path => Field (subst x es e) path
+  | Retag e kind call => Retag (subst x es e) kind (subst x es call)
+  | Let x1 e1 e2 =>
+      Let x1 (subst x es e1)
+                 (if bool_decide (BNamed x ≠ x1) then subst x es e2 else e2)
+  | Case e el => Case (subst x es e) (map (subst x es) el)
+  (* | Fork e => Fork (subst x es e) *)
+  (* | SysCall id => SysCall id *)
+  end.
+
+(* formal argument list substitution *)
+Definition subst' (mx : binder) (es : expr) : expr → expr :=
+  match mx with BNamed x => subst x es | BAnon => id end.
+
+Fixpoint subst_l (xl : list binder) (esl : list expr) (e : expr) : option expr :=
+  match xl, esl with
+  | [], [] => Some e
+  | x::xl, es::esl => subst' x es <$> subst_l xl esl e
+  | _, _ => None
+  end.
+Arguments subst_l _%binder _ _%E.
+
+Definition subst_v (xl : list binder) (vsl : vec val (length xl))
+                   (e : expr) : expr :=
+  Vector.fold_right2 (λ b, subst' b ∘ of_val) e _ (list_to_vec xl) vsl.
+Arguments subst_v _%binder _ _%E.
+
+Lemma subst_v_eq (xl : list binder) (vsl : vec val (length xl)) e :
+  Some $ subst_v xl vsl e = subst_l xl (of_val <$> vec_to_list vsl) e.
+Proof.
+  revert vsl. induction xl=>/= vsl; inv_vec vsl=>//=v vsl. by rewrite -IHxl.
+Qed.
+
+(** Evaluation contexts *)
+Inductive ectx_item :=
+(* | AppLCtx (el : list expr) *)
+(* | AppRCtx (v : val) (vl : list val) (el : list expr) *)
+| CallLCtx (el: list expr)
+| CallRCtx (v : val) (vl : list val) (el : list expr)
+| EndCallCtx
+| BinOpLCtx (op : bin_op) (e2 : expr)
+| BinOpRCtx (op : bin_op) (v1 : val)
+| TValCtx (vl : list val) (el : list expr)
+| ProjLCtx (e : expr)
+| ProjRCtx (v : val)
+| ConcLCtx (e : expr)
+| ConcRCtx (v : val)
+| CopyCtx
+| WriteLCtx (e : expr)
+| WriteRCtx (v : val)
+| FreeCtx
+(* | CasLCtx (e1 e2: expr) *)
+(* | CasMCtx (v0 : val) (e2 : expr) *)
+(* | CasRCtx (v0 : val) (v1 : val) *)
+(* | AtRdCtx *)
+(* | AtWrLCtx (e : expr) *)
+(* | AtWrRCtx (v : val) *)
+| DerefCtx (T: type)
+| RefCtx
+| FieldCtx (path : list nat)
+| RetagLCtx (kind: retag_kind) (call: expr)
+| RetagRCtx (v: val) (kind: retag_kind)
+| LetCtx (x: binder) (e2: expr)
+| CaseCtx (el : list expr).
+
+Definition fill_item (Ki : ectx_item) (e : expr) : expr :=
+  match Ki with
+  (* | AppLCtx el => App e el *)
+  (* | AppRCtx v vl el => App (of_val v) ((of_val <$> vl) ++ e :: el) *)
+  | CallLCtx el => Call e el
+  | CallRCtx v vl el => Call (of_val v) ((of_val <$> vl) ++ e :: el)
+  | EndCallCtx => EndCall e
+  | BinOpLCtx op e2 => BinOp op e e2
+  | BinOpRCtx op v1 => BinOp op (of_val v1) e
+  | TValCtx vl el => TVal ((of_val <$> vl) ++ e :: el)
+  | ProjLCtx e2 => Proj e e2
+  | ProjRCtx v1 => Proj (of_val v1) e
+  | ConcLCtx e2 => Conc e e2
+  | ConcRCtx v1 => Conc (of_val v1) e
+  | CopyCtx => Copy e
+  | WriteLCtx e2 => Write e e2
+  | WriteRCtx v1 => Write (of_val v1) e
+  | FreeCtx => Free e
+  (* | CasLCtx e1 e2 => CAS e e1 e2 *)
+  (* | CasMCtx v0 e2 => CAS (of_val v0) e e2 *)
+  (* | CasRCtx v0 v1 => CAS (of_val v0) (of_val v1) e *)
+  (* | AtRdCtx => AtomRead e *)
+  (* | AtWrLCtx e2 => AtomWrite e e2 *)
+  (* | AtWrRCtx v1 => AtomWrite (of_val v1) e *)
+  | DerefCtx T => Deref e T
+  | RefCtx => Ref e
+  | FieldCtx path => Field e path
+  | RetagLCtx kind call => Retag e kind call
+  | RetagRCtx v kind => Retag (of_val v) kind e
+  | LetCtx x e2 => Let x e e2
+  | CaseCtx el => Case e el
+  end.
+
+(** The stepping relation *)
+(* Be careful to make sure that poison is always stuck when used for anything
+   except for reading from or writing to memory! *)
+Definition Z_of_bool (b : bool) : Z :=
+  if b then 1 else 0.
+
+Definition lit_of_bool (b : bool) : lit :=
+  LitInt $ Z_of_bool b.
+
+Coercion lit_of_bool : bool >-> lit.
+Coercion LitInt : Z >-> lit.
+
+Implicit Type (h: mem).
+
+Fixpoint init_mem (l:loc) (n:nat) h : mem :=
+  match n with
+  | O => h
+  | S n => <[l := LitPoison]>(init_mem (l +ₗ 1) n h)
+  end.
+
+Fixpoint free_mem (l:loc) (n:nat) h : mem :=
+  match n with
+  | O => h
+  | S n => delete l (free_mem (l +ₗ 1) n h)
+  end.
+
+Inductive lit_eq h : lit → lit → Prop :=
+(* No refl case for poison *)
+| IntRefl z : lit_eq h (LitInt z) (LitInt z)
+| LocRefl l tag1 tag2 : lit_eq h (LitLoc l tag1) (LitLoc l tag2)
+(* Comparing unallocated pointers can non-deterministically say they are equal
+   even if they are not.  Given that our `free` actually makes addresses
+   re-usable, this may not be strictly necessary, but it is the most
+   conservative choice that avoids UB (and we cannot use UB as this operation is
+   possible in safe Rust).  See
+   <https://internals.rust-lang.org/t/comparing-dangling-pointers/3019> for some
+   more background. *)
+| LocUnallocL l1 l2 tag1 tag2 :
+    h !! l1 = None →
+    lit_eq h (LitLoc l1 tag1) (LitLoc l2 tag2)
+| LocUnallocR l1 l2 tag1 tag2 :
+    h !! l2 = None →
+    lit_eq h (LitLoc l1 tag1) (LitLoc l2 tag2).
+
+Inductive lit_neq : lit → lit → Prop :=
+| IntNeq z1 z2 :
+    z1 ≠ z2 → lit_neq (LitInt z1) (LitInt z2)
+| LocNeq l1 l2 tag1 tag2 :
+    l1 ≠ l2 → lit_neq (LitLoc l1 tag1) (LitLoc l2 tag2)
+| LocNeqNullR l tag :
+    lit_neq (LitLoc l tag) (LitInt 0)
+| LocNeqNullL l tag :
+    lit_neq (LitInt 0) (LitLoc l tag).
+
+Inductive bin_op_eval h : bin_op → lit → lit → lit → Prop :=
+| BinOpPlus z1 z2 :
+    bin_op_eval h AddOp (LitInt z1) (LitInt z2) (LitInt (z1 + z2))
+| BinOpMinus z1 z2 :
+    bin_op_eval h SubOp (LitInt z1) (LitInt z2) (LitInt (z1 - z2))
+| BinOpLe z1 z2 :
+    bin_op_eval h LeOp (LitInt z1) (LitInt z2) (lit_of_bool $ bool_decide (z1 ≤ z2))
+| BinOpLt z1 z2 :
+    bin_op_eval h LtOp (LitInt z1) (LitInt z2) (lit_of_bool $ bool_decide (z1 < z2))
+| BinOpEqTrue l1 l2 :
+    lit_eq h l1 l2 → bin_op_eval h EqOp l1 l2 (lit_of_bool true)
+| BinOpEqFalse l1 l2 :
+    lit_neq l1 l2 → bin_op_eval h EqOp l1 l2 (lit_of_bool false)
+| BinOpOffset l z tag :
+    bin_op_eval h OffsetOp (LitLoc l tag) (LitInt z) (LitLoc (l +ₗ z) tag).
+
+(* Compute subtype of `T` and offset to it from `path` *)
+Fixpoint field_access (T: type) (path : list nat) :
+  option (nat * type) :=
+  match path with
+  | [] => Some (O, T)
+  | i :: path =>
+    match T with
+    | Scalar sz =>
+        if bool_decide (i ≤ sz) then Some (i, Scalar (sz - i)) else None
+    | Reference _ _ => match i with O => Some (O, T) | _ => None end
+    | Unsafe T => field_access T path
+    | Union Ts => T ← Ts !! i ; field_access T path
+    | Product Ts =>
+        T ← Ts !! i ; offT ← field_access T path;
+        let sz : nat := foldl (λ sz T', sz + tsize T')%nat O (take i Ts) in
+        Some (offT.1 + sz, offT.2)%nat
+    | Sum Ts =>
+        T ← Ts !! i ; offT ← field_access T path; Some (offT.1 + 1, offT.2)%nat
+    end
+  end.
+
+Fixpoint write_mem l (vl: list lit) h: mem :=
+  match vl with
+  | [] => h
+  | v :: vl => write_mem (l +ₗ 1) vl (<[l := v]> h)
+  end.
+
+Equations read_mem (l: loc) (n: nat) h: option (list lit) :=
+  read_mem l n h := go l n (Some [])
+  where go : loc → nat → option (list lit) → option (list lit) :=
+        go l O      oacc := oacc;
+        go l (S n)  oacc :=
+          acc ← oacc ;
+          v ← h !! l;
+          go (l +ₗ 1) n (Some (acc ++ [v])).
+
+Inductive expr_step (FNs: fn_env):
+  expr → mem → mem_event → expr → mem → list expr → Prop :=
+| BinOpBS op l1 l2 l' h :
+    bin_op_eval h op l1 l2 l' →
+    expr_step FNs (BinOp op (#[ #l1]) (#[ #l2])) h SilentEvt (#[ #l']) h []
+(* | BetaBS f xl e e' el h :
+    Forall (λ ei, is_Some (to_val ei)) el →
+    Closed (f :b: xl +b+ []) e →
+    subst_l (f::xl) (Rec f xl e :: el) e = Some e' →
+    expr_step (App (Rec f xl e) el) h SilentEvt e' h [] *)
+| CallBS name (call: call_id) el h xl e HC e':
+    FNs !! name = Some (@FunV xl e HC) →
+    Forall (λ ei, is_Some (to_val ei)) el →
+    subst_l xl el e = Some e' →
+    expr_step FNs (Call (#(LitFnPtr name)) el) h
+                  (NewCallEvt name call)
+                  (let ret := e' in EndCall #(LitCall call) ;; ret) h []
+| EndCallBS (call: call_id) h:
+    expr_step FNs (EndCall #(LitCall call)) h (EndCallEvt call) #☠ h []
+(* TODO: add more operations for tempvalue lists *)
+| ProjBS h el (i: Z) vl v
+    (DEFINED: 0 ≤ i ∧ vl !! (Z.to_nat i) = Some v)
+    (VALUES: to_val (TVal el) = Some (TValV vl)) :
+    expr_step FNs (Proj (TVal el) #i) h SilentEvt #v h []
+| ConcBS h el1 el2 vl1 vl2
+    (VALUES1: to_val (TVal el1) = Some (TValV vl1))
+    (VALUES2: to_val (TVal el2) = Some (TValV vl2)) :
+    expr_step FNs (Conc (TVal el1) (TVal el2)) h
+              SilentEvt (of_val (TValV (vl1 ++ vl2))) h []
+| CopyBS l lbor T (vl: list lit) h
+    (READ: read_mem l (tsize T) h = Some vl)
+    (* (LEN: length vl = tsize T) *)
+    (* (VALUES: ∀ (i: nat), (i < length vl)%nat → h !! (l +ₗ i) = vl !! i) *) :
+    expr_step FNs (Copy (Place l lbor T)) h
+              (CopyEvt l lbor T vl)
+              (of_val (TValV vl)) h
+              []
+| WriteBS l lbor T el vl h (LENe: length vl = tsize T)
+    (DEFINED: ∀ (i: nat), (i < length vl)%nat → l +ₗ i ∈ dom (gset loc) h)
+    (VALUES: to_val (TVal el) = Some (TValV vl)) :
+    expr_step FNs (Place l lbor T <- TVal el) h
+              (WriteEvt l lbor T vl)
+              #☠ (write_mem l vl h)
+              []
+| AllocBS l lbor T h :
+    (∀ m, h !! (l +ₗ m) = None) →
+    expr_step FNs (Alloc T) h
+              (AllocEvt l lbor T)
+              (Place l lbor T) (init_mem l (tsize T) h)
+              []
+| DeallocBS T l lbor h :
+    (∀ m, is_Some (h !! (l +ₗ m)) ↔ 0 ≤ m < tsize T) →
+    expr_step FNs (Free (Place l lbor T)) h
+              (DeallocEvt l lbor T)
+              #☠ (free_mem l (tsize T) h)
+              []
+| RefBS l lbor T h :
+    is_Some (h !! l) →
+    expr_step FNs (Ref (Place l lbor T)) h SilentEvt #(LitLoc l lbor) h []
+| DerefBS l lbor T h
+    (DEFINED: ∀ (i: nat), (i < tsize T)%nat → l +ₗ i ∈ dom (gset loc) h) :
+    expr_step FNs ( *{T} #(LitLoc l lbor)) h
+              SilentEvt
+              (Place l lbor T) h
+              []
+| FieldBS l lbor T path off T' h
+    (FIELD: field_access T path = Some (off, T')) :
+    expr_step FNs (Field (Place l lbor T) path) h
+              SilentEvt (Place (l +ₗ off) lbor T') h []
+| RetagBS x xbor T kind kind' h e v
+    (VAL: to_val e = Some v)
+    (KIND: match kind with
+           | FnEntry _ => ∃ call, v = LitV $ LitInt call ∧
+                          0 ≤ call ∧ kind' = FnEntry (Z.to_nat call)
+           | _ => kind' = kind
+           end) :
+    expr_step FNs (Retag (Place x xbor T) kind e) h
+              (RetagEvt x T kind') (Lit LitPoison) h []
+| LetBS x e1 e2 h e' :
+    is_Some (to_val e1) →
+    subst x e2 e1 = e' →
+    expr_step FNs (let x := e1 in e2) h SilentEvt e' h []
+| CaseBS i el e h :
+    0 ≤ i →
+    el !! (Z.to_nat i) = Some e →
+    expr_step FNs (case: #i of el) h SilentEvt e h []
+(* | ForkBS e h:
+    expr_step (Fork e) h SilentEvt (Lit LitPoison) h [e] *)
+(* observable behavior *)
+(* | SysCallBS id h:
+    expr_step (SysCall id) h (SysCallEvt id) (Lit LitPoison) h [] *).
