theories/lang_base.v
@@ -1,0 +1,285 @@
+From Coq Require Export ssreflect.
+From stdpp Require Export countable binders gmap.
+
+Global Open Scope general_if_scope.
+
+From stbor Require Export type.
+Set Default Proof Using "Type".
+
+Delimit Scope loc_scope with L.
+Delimit Scope expr_scope with E.
+Delimit Scope val_scope with V.
+
+Open Scope Z_scope.
+
+(** Locations *)
+Definition block : Set := positive.
+Definition loc : Set := block * Z.
+
+Bind Scope loc_scope with loc.
+Open Scope loc_scope.
+
+Definition shift_loc (l : loc) (z : Z) : loc := (l.1, l.2 + z).
+
+Notation "l +ₗ z" := (shift_loc l%L z%Z)
+  (at level 50, left associativity) : loc_scope.
+
+(** Shifting for locations *)
+Lemma shift_loc_assoc l n n' : l +ₗ n +ₗ n' = l +ₗ (n + n').
+Proof. rewrite /shift_loc /=. f_equal. lia. Qed.
+Lemma shift_loc_0 l : l +ₗ 0 = l.
+Proof. destruct l as [b o]. rewrite /shift_loc /=. f_equal. lia. Qed.
+
+Lemma shift_loc_assoc_nat l (n n' : nat) : l +ₗ n +ₗ n' = l +ₗ (n + n')%nat.
+Proof. rewrite /shift_loc /=. f_equal. lia. Qed.
+Lemma shift_loc_0_nat l : l +ₗ 0%nat = l.
+Proof. destruct l as [b o]. rewrite /shift_loc /=. f_equal. lia. Qed.
+
+Instance shift_loc_inj l : Inj (=) (=) (shift_loc l).
+Proof. destruct l as [b o]; intros n n' [=?]; lia. Qed.
+
+Lemma shift_loc_block l n : (l +ₗ n).1 = l.1.
+Proof. done. Qed.
+
+(** Protector tracker: track if a call_id is active,
+  i.e. the call is still in the call stack *)
+Notation call_id := nat (only parsing).
+Definition protectors := gmap call_id bool.
+
+(** Tags for pointers *)
+Notation ptr_id := nat (only parsing).
+
+Inductive tag :=
+  | Tagged (t: ptr_id)
+  | Untagged
+  .
+
+Instance tag_eq_dec : EqDecision tag.
+Proof. solve_decision. Defined.
+Instance tag_countable : Countable tag.
+Proof.
+  refine (inj_countable
+          (λ tg, match tg with
+              | Tagged t => inl t
+              | Untagged => inr ()
+              end)
+          (λ s, match s with
+              | inl t => Some $ Tagged t
+              | inr _ => Some $ Untagged
+              end) _); by intros [].
+Qed.
+
+Inductive permission := Unique | SharedReadWrite | SharedReadOnly | Disabled.
+Instance permission_eq_dec : EqDecision permission.
+Proof. solve_decision. Defined.
+Instance permission_countable : Countable permission.
+Proof.
+  refine (inj_countable
+    (λ p,
+      match p with
+      | Unique => 0 | SharedReadWrite => 1 | SharedReadOnly => 2 | Disabled => 3
+      end)
+    (λ s,
+      match s with
+      | 0 => Some Unique | 1 => Some SharedReadWrite | 2 => Some SharedReadOnly
+      | _ => Some Disabled
+      end) _); by intros [].
+Qed.
+
+(** Stacks of borrows. *)
+Record item := mkItem {
+  perm      : permission;
+  tg        : tag;
+  protector : option call_id;
+}.
+Instance item_eq_dec : EqDecision item.
+Proof. solve_decision. Defined.
+
+Definition stack := list item.
+Definition stacks := gmap loc stack.
+
+(** Retag kinds *)
+Inductive retag_kind := FnEntry (c: call_id) | TwoPhase | RawRt | Default.
+
+Definition is_two_phase (kind: retag_kind) : bool :=
+  match kind with TwoPhase => true | _ => false end.
+Definition adding_protector (kind: retag_kind) : option call_id :=
+  match kind with FnEntry c => Some c | _ => None end.
+
+(** Language base constructs -------------------------------------------------*)
+
+(** Unary/Binary ops *)
+Inductive bin_op :=
+  | AddOp     (* + addition       *)
+  | SubOp     (* - subtraction    *)
+(* | MulOp     (* * multiplication *)
+  | DivOp     (* / division       *)
+  | RemOp     (* % modulus        *)
+  | BitXorOp  (* ^ bit xor        *)
+  | BitAndOp  (* & bit and        *)
+  | BitOrOp   (* | bit or         *)
+  | ShlOp     (* << shift left    *)
+  | ShrOp     (* >> shift right   *) *)
+  | EqOp      (* == equality      *)
+  | LtOp      (* < less than      *)
+  | LeOp      (* <= less than or equal to *)
+(* | NeOp      (* != not equal to  *)
+  | GeOp      (* >= greater than or equal to *)
+  | GtOp      (* > greater than   *) *)
+  | OffsetOp  (* . offset         *)
+  .
+
+(** Base values *)
+Inductive lit :=
+  | LitPoison | LitLoc (l: loc) (tg: tag) | LitInt (n : Z)
+  | LitFnPtr (name: string)
+  | LitCall (id: call_id).
+
+(** Expressions *)
+Inductive expr :=
+(* base values *)
+| Lit (l: lit)
+(* variables *)
+| Var (x : string)
+(* | App (e : expr) (el: list expr) *)
+(* | Rec (f : binder) (xl : list binder) (e : expr) *)
+(* function calls *)
+| Call (e: expr) (el: list expr) (* Call a function through a FnPtr `e`
+                                    with arguments `el` *)
+(* function call tracking *)
+| EndCall (e: expr)               (* End the call with id `e` *)
+(* temp values *)
+| TVal (el: list expr)
+| Proj (e1 e2 : expr)
+| Conc (e1 e2: expr)
+(* bin op *)
+| BinOp (op : bin_op) (e1 e2 : expr)
+(* place operation *)
+| Place (l: loc) (tg: tag) (T: type)
+                                  (* A place is a tagged pointer: every access
+                                     to memory revolves around a place. *)
+| Deref (e: expr) (T: type)       (* Deference a pointer `e` into a place
+                                     presenting the location that `e` points to.
+                                     The location has type `T`. *)
+| Ref (e: expr)                   (* Turn a place `e` into a pointer value. *)
+| Field (e: expr) (path: list nat)(* Create a place that points to a component
+                                     of the place `e`. `path` defines the path
+                                     through the type. *)
+(* mem op *)
+| Copy (e : expr)                 (* Read from the place `e` *)
+| Write (e1 e2: expr)             (* Write the value `e2` to the place `e1` *)
+| Alloc (T: type)                 (* Allocate a place of type `T` *)
+| Free (e : expr)                 (* Free the place `e` *)
+(* atomic mem op *)
+(* | CAS (e0 e1 e2 : expr) *)     (* CAS the value `e2` for `e1` to the place `e0` *)
+(* | AtomWrite (e1 e2: expr) *)
+(* | AtomRead (e: expr) *)
+(* retag *)
+| Retag (e : expr) (kind: retag_kind) (call_id: expr)
+                                  (* Retag the place `e` with retag kind `kind`. *)
+(* let binding *)
+| Let (x : binder) (e1 e2: expr)
+(* case *)
+| Case (e : expr) (el: list expr)
+(* concurrency *)
+(* | Fork (e : expr) *)
+(* observable behavior *)
+(* | SysCall (id: nat) *)
+.
+
+Bind Scope expr_scope with expr.
+
+(* Arguments App _%E _%E. *)
+Arguments BinOp _ _%E _%E.
+Arguments Call _%E _%E.
+Arguments EndCall _%E.
+Arguments TVal _%E.
+Arguments Proj _%E _%E.
+Arguments Conc _%E _%E.
+Arguments Deref _%E _%T.
+Arguments Ref _%E.
+Arguments Field _%E _.
+Arguments Copy _%E.
+Arguments Write _%E _%E.
+Arguments Alloc _%T.
+Arguments Free _%E.
+(* Arguments CAS _%E _%E _%E. *)
+(* Arguments AtomWrite _%E _%E. *)
+(* Arguments AtomRead _%E. *)
+Arguments Retag _%E _ _%E.
+Arguments Let _%binder _%E _%E.
+Arguments Case _%E _%E.
+(* Arguments Fork _%E. *)
+
+(** Closedness *)
+Fixpoint is_closed (X : list string) (e : expr) : bool :=
+  match e with
+  | Lit _ | Place _ _ _ | Alloc _ (* | SysCall _ *) => true
+  | Var x => bool_decide (x ∈ X)
+  (* | Rec f xl e => is_closed (f :b: xl +b+ X) e *)
+  | BinOp _ e1 e2 | (* AtomWrite e1 e2 | *) Write e1 e2 | Retag e1 _ e2
+      | Conc e1 e2 | Proj e1 e2 => is_closed X e1 && is_closed X e2
+  | TVal el => forallb (is_closed X) el
+  | Let x e1 e2 => is_closed X e1 && is_closed (x :b: X) e2
+  | Case e el | Call e el (* | App e el  *) => is_closed X e && forallb (is_closed X) el
+  | Copy e | Deref e _ | Ref e | Field e _
+      | Free e | EndCall e (* | AtomRead e | Fork e *) => is_closed X e
+  (* | CAS e0 e1 e2 => is_closed X e0 && is_closed X e1 && is_closed X e2 *)
+  end.
+
+Class Closed (X : list string) (e : expr) := closed : is_closed X e.
+Instance closed_proof_irrel env e : ProofIrrel (Closed env e).
+Proof. rewrite /Closed. apply _. Qed.
+Instance closed_decision env e : Decision (Closed env e).
+Proof. rewrite /Closed. apply _. Qed.
+
+(** Irreducible (language values) *)
+Inductive val :=
+| LitV (v : lit)
+| TValV (vl : list lit)
+| PlaceV (l: loc) (tg: tag) (T: type)
+.
+Bind Scope val_scope with val.
+
+Definition of_val (v : val) : expr :=
+  match v with
+  | LitV v => Lit v
+  | TValV vl => TVal (Lit <$> vl)
+  | PlaceV l tag T => Place l tag T
+  end.
+
+Definition to_lit (e: expr): option lit :=
+  match e with
+  | Lit l => Some l
+  | _ => None
+  end.
+Definition to_lits (vl : list lit) (el: list expr) : option (list lit) :=
+  foldl (λ acc e, vl ← acc; v ← to_lit e; Some (vl ++ [v])) (Some vl) el.
+Definition to_val (e : expr) : option val :=
+  match e with
+  | Lit v => Some (LitV v)
+  | Place l T tag => Some (PlaceV l T tag)
+  | TVal el => vl ← to_lits [] el; Some (TValV vl)
+  | _ => None
+  end.
+
+(** Global static function table *)
+Inductive function :=
+| FunV (xl : list binder) (e : expr) `{Closed (xl +b+ []) e}.
+Definition fn_env := gmap string function.
+
+(** Main state: a heap of literals. *)
+Definition mem := gmap loc lit.
+
+(** Internal memory events *)
+Inductive mem_event :=
+| AllocEvt (l : loc) (lbor: tag) (T: type)
+| DeallocEvt (l: loc) (lbor: tag) (T: type)
+| CopyEvt (l: loc) (lbor: tag) (T: type) (vl: list lit)
+| WriteEvt (l: loc) (lbor: tag) (T: type) (vl: list lit)
+| NewCallEvt (name: string) (call: call_id)
+| EndCallEvt (call: call_id)
+| RetagEvt (x: loc) (T: type) (kind: retag_kind)
+(* | SysCallEvt (id: nat) *)
+| SilentEvt
+.
